make ett_inf.v & ett_ott.v compile

src/FcEtt/ett_ott.v
@@ -1,5 +1,7 @@
 Require Import Bool.
 Require Import Metalib.Metatheory.
+Require Export FcEtt.grade_sig.
+
 (** syntax *)
 Definition tmvar : Set := var. (*r variables *)
 Definition covar : Set := var. (*r coercion variables *)
@@ -8,9 +10,7 @@ Definition const : Set := atom.
 Definition tyfam : Set := atom.
 Definition index : Set := nat. (*r indices *)
 
-Inductive relflag : Set :=  (*r relevance flag *)
- | Rel : relflag
- | Irrel : relflag.
+Definition grade : Set := grade.
 
 Inductive constraint : Set :=  (*r props *)
  | Eq (a:tm) (b:tm) (A:tm)
@@ -19,18 +19,17 @@ with tm : Set :=  (*r types and kinds *)
  | a_Star : tm
  | a_Var_b (_:nat)
  | a_Var_f (x:tmvar)
- | a_Abs (rho:relflag) (A:tm) (b:tm)
- | a_UAbs (rho:relflag) (b:tm)
- | a_App (a:tm) (rho:relflag) (b:tm)
+ | a_Abs (psi:grade) (A:tm) (b:tm)
+ | a_UAbs (psi:grade) (b:tm)
+ | a_App (a:tm) (psi:grade) (b:tm)
  | a_Fam (F:tyfam)
  | a_Const (T:const)
- | a_Pi (rho:relflag) (A:tm) (B:tm)
+ | a_Pi (psi:grade) (A:tm) (B:tm)
  | a_Conv (a:tm) (g:co)
- | a_CPi (phi:constraint) (B:tm)
- | a_CAbs (phi:constraint) (b:tm)
- | a_UCAbs (b:tm)
+ | a_CPi (psi:grade) (phi:constraint) (B:tm)
+ | a_CAbs (psi:grade) (phi:constraint) (b:tm)
+ | a_UCAbs (psi:grade) (b:tm)
  | a_CApp (a:tm) (g:co)
- | a_Bullet : tm
  | a_DataCon (K:datacon)
  | a_Case (a:tm) (brs5:brs)
 with brs : Set :=  (*r case branches *)
@@ -45,15 +44,15 @@ with co : Set :=  (*r explicit coercions *)
  | g_Refl2 (a:tm) (b:tm) (g:co)
  | g_Sym (g:co)
  | g_Trans (g1:co) (g2:co)
- | g_PiCong (rho:relflag) (g1:co) (g2:co)
- | g_AbsCong (rho:relflag) (g1:co) (g2:co)
- | g_AppCong (g1:co) (rho:relflag) (g2:co)
+ | g_PiCong (psi:grade) (g1:co) (g2:co)
+ | g_AbsCong (psi:grade) (g1:co) (g2:co)
+ | g_AppCong (g1:co) (psi:grade) (g2:co)
  | g_PiFst (g:co)
  | g_CPiFst (g:co)
  | g_IsoSnd (g:co)
  | g_PiSnd (g1:co) (g2:co)
  | g_CPiCong (g1:co) (g3:co)
- | g_CAbsCong (g1:co) (g3:co) (g4:co)
+ | g_CAbsCong (psi:grade) (g1:co) (g3:co) (g4:co)
  | g_CAppCong (g:co) (g1:co) (g2:co)
  | g_CPiSnd (g:co) (g1:co) (g2:co)
  | g_Cast (g1:co) (g2:co)
@@ -63,19 +62,22 @@ with co : Set :=  (*r explicit coercions *)
  | g_Left (g:co) (g':co)
  | g_Right (g:co) (g':co).
 
+Definition econtext : Set := list ( atom * grade ).
+
 Inductive sort : Set :=  (*r binding classifier *)
  | Tm (A:tm)
  | Co (phi:constraint).
+
+
+Definition context : Set := list ( atom * (grade * sort) ).
+
 
 Inductive sig_sort : Set :=  (*r signature classifier *)
  | Cs (A:tm)
  | Ax (a:tm) (A:tm).
 
-Definition context : Set := list ( atom * sort ).
-
-Definition available_props : Type := atoms.
-
 Definition sig : Set := list (atom * sig_sort).
+
 
 (* EXPERIMENTAL *)
 (** auxiliary functions on the new list types *)
@@ -98,15 +100,15 @@ Fixpoint open_co_wrt_co_rec (k:nat) (g_5:co) (g__6:co) {struct g__6}: co :=
   | (g_Refl2 a b g) => g_Refl2 (open_tm_wrt_co_rec k g_5 a) (open_tm_wrt_co_rec k g_5 b) (open_co_wrt_co_rec k g_5 g)
   | (g_Sym g) => g_Sym (open_co_wrt_co_rec k g_5 g)
   | (g_Trans g1 g2) => g_Trans (open_co_wrt_co_rec k g_5 g1) (open_co_wrt_co_rec k g_5 g2)
-  | (g_PiCong rho g1 g2) => g_PiCong rho (open_co_wrt_co_rec k g_5 g1) (open_co_wrt_co_rec k g_5 g2)
-  | (g_AbsCong rho g1 g2) => g_AbsCong rho (open_co_wrt_co_rec k g_5 g1) (open_co_wrt_co_rec k g_5 g2)
-  | (g_AppCong g1 rho g2) => g_AppCong (open_co_wrt_co_rec k g_5 g1) rho (open_co_wrt_co_rec k g_5 g2)
+  | (g_PiCong psi g1 g2) => g_PiCong psi (open_co_wrt_co_rec k g_5 g1) (open_co_wrt_co_rec k g_5 g2)
+  | (g_AbsCong psi g1 g2) => g_AbsCong psi (open_co_wrt_co_rec k g_5 g1) (open_co_wrt_co_rec k g_5 g2)
+  | (g_AppCong g1 psi g2) => g_AppCong (open_co_wrt_co_rec k g_5 g1) psi (open_co_wrt_co_rec k g_5 g2)
   | (g_PiFst g) => g_PiFst (open_co_wrt_co_rec k g_5 g)
   | (g_CPiFst g) => g_CPiFst (open_co_wrt_co_rec k g_5 g)
   | (g_IsoSnd g) => g_IsoSnd (open_co_wrt_co_rec k g_5 g)
   | (g_PiSnd g1 g2) => g_PiSnd (open_co_wrt_co_rec k g_5 g1) (open_co_wrt_co_rec k g_5 g2)
   | (g_CPiCong g1 g3) => g_CPiCong (open_co_wrt_co_rec k g_5 g1) (open_co_wrt_co_rec (S k) g_5 g3)
-  | (g_CAbsCong g1 g3 g4) => g_CAbsCong (open_co_wrt_co_rec k g_5 g1) (open_co_wrt_co_rec (S k) g_5 g3) (open_co_wrt_co_rec k g_5 g4)
+  | (g_CAbsCong psi g1 g3 g4) => g_CAbsCong psi (open_co_wrt_co_rec k g_5 g1) (open_co_wrt_co_rec (S k) g_5 g3) (open_co_wrt_co_rec k g_5 g4)
   | (g_CAppCong g g1 g2) => g_CAppCong (open_co_wrt_co_rec k g_5 g) (open_co_wrt_co_rec k g_5 g1) (open_co_wrt_co_rec k g_5 g2)
   | (g_CPiSnd g g1 g2) => g_CPiSnd (open_co_wrt_co_rec k g_5 g) (open_co_wrt_co_rec k g_5 g1) (open_co_wrt_co_rec k g_5 g2)
   | (g_Cast g1 g2) => g_Cast (open_co_wrt_co_rec k g_5 g1) (open_co_wrt_co_rec k g_5 g2)
@@ -126,18 +128,17 @@ with open_tm_wrt_co_rec (k:nat) (g5:co) (a5:tm) {struct a5}: tm :=
   | a_Star => a_Star 
   | (a_Var_b nat) => a_Var_b nat
   | (a_Var_f x) => a_Var_f x
-  | (a_Abs rho A b) => a_Abs rho (open_tm_wrt_co_rec k g5 A) (open_tm_wrt_co_rec k g5 b)
-  | (a_UAbs rho b) => a_UAbs rho (open_tm_wrt_co_rec k g5 b)
-  | (a_App a rho b) => a_App (open_tm_wrt_co_rec k g5 a) rho (open_tm_wrt_co_rec k g5 b)
+  | (a_Abs psi A b) => a_Abs psi (open_tm_wrt_co_rec k g5 A) (open_tm_wrt_co_rec k g5 b)
+  | (a_UAbs psi b) => a_UAbs psi (open_tm_wrt_co_rec k g5 b)
+  | (a_App a psi b) => a_App (open_tm_wrt_co_rec k g5 a) psi (open_tm_wrt_co_rec k g5 b)
   | (a_Fam F) => a_Fam F
   | (a_Const T) => a_Const T
-  | (a_Pi rho A B) => a_Pi rho (open_tm_wrt_co_rec k g5 A) (open_tm_wrt_co_rec k g5 B)
+  | (a_Pi psi A B) => a_Pi psi (open_tm_wrt_co_rec k g5 A) (open_tm_wrt_co_rec k g5 B)
   | (a_Conv a g) => a_Conv (open_tm_wrt_co_rec k g5 a) (open_co_wrt_co_rec k g5 g)
-  | (a_CPi phi B) => a_CPi (open_constraint_wrt_co_rec k g5 phi) (open_tm_wrt_co_rec (S k) g5 B)
-  | (a_CAbs phi b) => a_CAbs (open_constraint_wrt_co_rec k g5 phi) (open_tm_wrt_co_rec (S k) g5 b)
-  | (a_UCAbs b) => a_UCAbs (open_tm_wrt_co_rec (S k) g5 b)
+  | (a_CPi psi phi B) => a_CPi psi (open_constraint_wrt_co_rec k g5 phi) (open_tm_wrt_co_rec (S k) g5 B)
+  | (a_CAbs psi phi b) => a_CAbs psi (open_constraint_wrt_co_rec k g5 phi) (open_tm_wrt_co_rec (S k) g5 b)
+  | (a_UCAbs psi b) => a_UCAbs psi (open_tm_wrt_co_rec (S k) g5 b)
   | (a_CApp a g) => a_CApp (open_tm_wrt_co_rec k g5 a) (open_co_wrt_co_rec k g5 g)
-  | a_Bullet => a_Bullet 
   | (a_DataCon K) => a_DataCon K
   | (a_Case a brs5) => a_Case (open_tm_wrt_co_rec k g5 a) (open_brs_wrt_co_rec k g5 brs5)
 end
@@ -157,15 +158,15 @@ Fixpoint open_co_wrt_tm_rec (k:nat) (a5:tm) (g_5:co) {struct g_5}: co :=
   | (g_Refl2 a b g) => g_Refl2 (open_tm_wrt_tm_rec k a5 a) (open_tm_wrt_tm_rec k a5 b) (open_co_wrt_tm_rec k a5 g)
   | (g_Sym g) => g_Sym (open_co_wrt_tm_rec k a5 g)
   | (g_Trans g1 g2) => g_Trans (open_co_wrt_tm_rec k a5 g1) (open_co_wrt_tm_rec k a5 g2)
-  | (g_PiCong rho g1 g2) => g_PiCong rho (open_co_wrt_tm_rec k a5 g1) (open_co_wrt_tm_rec (S k) a5 g2)
-  | (g_AbsCong rho g1 g2) => g_AbsCong rho (open_co_wrt_tm_rec k a5 g1) (open_co_wrt_tm_rec (S k) a5 g2)
-  | (g_AppCong g1 rho g2) => g_AppCong (open_co_wrt_tm_rec k a5 g1) rho (open_co_wrt_tm_rec k a5 g2)
+  | (g_PiCong psi g1 g2) => g_PiCong psi (open_co_wrt_tm_rec k a5 g1) (open_co_wrt_tm_rec (S k) a5 g2)
+  | (g_AbsCong psi g1 g2) => g_AbsCong psi (open_co_wrt_tm_rec k a5 g1) (open_co_wrt_tm_rec (S k) a5 g2)
+  | (g_AppCong g1 psi g2) => g_AppCong (open_co_wrt_tm_rec k a5 g1) psi (open_co_wrt_tm_rec k a5 g2)
   | (g_PiFst g) => g_PiFst (open_co_wrt_tm_rec k a5 g)
   | (g_CPiFst g) => g_CPiFst (open_co_wrt_tm_rec k a5 g)
   | (g_IsoSnd g) => g_IsoSnd (open_co_wrt_tm_rec k a5 g)
   | (g_PiSnd g1 g2) => g_PiSnd (open_co_wrt_tm_rec k a5 g1) (open_co_wrt_tm_rec k a5 g2)
   | (g_CPiCong g1 g3) => g_CPiCong (open_co_wrt_tm_rec k a5 g1) (open_co_wrt_tm_rec k a5 g3)
-  | (g_CAbsCong g1 g3 g4) => g_CAbsCong (open_co_wrt_tm_rec k a5 g1) (open_co_wrt_tm_rec k a5 g3) (open_co_wrt_tm_rec k a5 g4)
+  | (g_CAbsCong psi g1 g3 g4) => g_CAbsCong psi (open_co_wrt_tm_rec k a5 g1) (open_co_wrt_tm_rec k a5 g3) (open_co_wrt_tm_rec k a5 g4)
   | (g_CAppCong g g1 g2) => g_CAppCong (open_co_wrt_tm_rec k a5 g) (open_co_wrt_tm_rec k a5 g1) (open_co_wrt_tm_rec k a5 g2)
   | (g_CPiSnd g g1 g2) => g_CPiSnd (open_co_wrt_tm_rec k a5 g) (open_co_wrt_tm_rec k a5 g1) (open_co_wrt_tm_rec k a5 g2)
   | (g_Cast g1 g2) => g_Cast (open_co_wrt_tm_rec k a5 g1) (open_co_wrt_tm_rec k a5 g2)
@@ -190,18 +191,17 @@ with open_tm_wrt_tm_rec (k:nat) (a5:tm) (a_6:tm) {struct a_6}: tm :=
         | inright _ => a_Var_b (nat - 1)
       end
   | (a_Var_f x) => a_Var_f x
-  | (a_Abs rho A b) => a_Abs rho (open_tm_wrt_tm_rec k a5 A) (open_tm_wrt_tm_rec (S k) a5 b)
-  | (a_UAbs rho b) => a_UAbs rho (open_tm_wrt_tm_rec (S k) a5 b)
-  | (a_App a rho b) => a_App (open_tm_wrt_tm_rec k a5 a) rho (open_tm_wrt_tm_rec k a5 b)
+  | (a_Abs psi A b) => a_Abs psi (open_tm_wrt_tm_rec k a5 A) (open_tm_wrt_tm_rec (S k) a5 b)
+  | (a_UAbs psi b) => a_UAbs psi (open_tm_wrt_tm_rec (S k) a5 b)
+  | (a_App a psi b) => a_App (open_tm_wrt_tm_rec k a5 a) psi (open_tm_wrt_tm_rec k a5 b)
   | (a_Fam F) => a_Fam F
   | (a_Const T) => a_Const T
-  | (a_Pi rho A B) => a_Pi rho (open_tm_wrt_tm_rec k a5 A) (open_tm_wrt_tm_rec (S k) a5 B)
+  | (a_Pi psi A B) => a_Pi psi (open_tm_wrt_tm_rec k a5 A) (open_tm_wrt_tm_rec (S k) a5 B)
   | (a_Conv a g) => a_Conv (open_tm_wrt_tm_rec k a5 a) (open_co_wrt_tm_rec k a5 g)
-  | (a_CPi phi B) => a_CPi (open_constraint_wrt_tm_rec k a5 phi) (open_tm_wrt_tm_rec k a5 B)
-  | (a_CAbs phi b) => a_CAbs (open_constraint_wrt_tm_rec k a5 phi) (open_tm_wrt_tm_rec k a5 b)
-  | (a_UCAbs b) => a_UCAbs (open_tm_wrt_tm_rec k a5 b)
+  | (a_CPi psi phi B) => a_CPi psi (open_constraint_wrt_tm_rec k a5 phi) (open_tm_wrt_tm_rec k a5 B)
+  | (a_CAbs psi phi b) => a_CAbs psi (open_constraint_wrt_tm_rec k a5 phi) (open_tm_wrt_tm_rec k a5 b)
+  | (a_UCAbs psi b) => a_UCAbs psi (open_tm_wrt_tm_rec k a5 b)
   | (a_CApp a g) => a_CApp (open_tm_wrt_tm_rec k a5 a) (open_co_wrt_tm_rec k a5 g)
-  | a_Bullet => a_Bullet 
   | (a_DataCon K) => a_DataCon K
   | (a_Case a brs5) => a_Case (open_tm_wrt_tm_rec k a5 a) (open_brs_wrt_tm_rec k a5 brs5)
 end
@@ -287,18 +287,18 @@ Inductive lc_co : co -> Prop :=    (* defn lc_co *)
      (lc_co g1) ->
      (lc_co g2) ->
      (lc_co (g_Trans g1 g2))
- | lc_g_PiCong : forall (rho:relflag) (g1 g2:co),
+ | lc_g_PiCong : forall (psi:grade) (g1 g2:co),
      (lc_co g1) ->
       ( forall x , lc_co  ( open_co_wrt_tm g2 (a_Var_f x) )  )  ->
-     (lc_co (g_PiCong rho g1 g2))
- | lc_g_AbsCong : forall (rho:relflag) (g1 g2:co),
+     (lc_co (g_PiCong psi g1 g2))
+ | lc_g_AbsCong : forall (psi:grade) (g1 g2:co),
      (lc_co g1) ->
       ( forall x , lc_co  ( open_co_wrt_tm g2 (a_Var_f x) )  )  ->
-     (lc_co (g_AbsCong rho g1 g2))
- | lc_g_AppCong : forall (g1:co) (rho:relflag) (g2:co),
+     (lc_co (g_AbsCong psi g1 g2))
+ | lc_g_AppCong : forall (g1:co) (psi:grade) (g2:co),
      (lc_co g1) ->
      (lc_co g2) ->
-     (lc_co (g_AppCong g1 rho g2))
+     (lc_co (g_AppCong g1 psi g2))
  | lc_g_PiFst : forall (g:co),
      (lc_co g) ->
      (lc_co (g_PiFst g))
@@ -316,11 +316,11 @@ Inductive lc_co : co -> Prop :=    (* defn lc_co *)
      (lc_co g1) ->
       ( forall c , lc_co  ( open_co_wrt_co g3 (g_Var_f c) )  )  ->
      (lc_co (g_CPiCong g1 g3))
- | lc_g_CAbsCong : forall (g1 g3 g4:co),
+ | lc_g_CAbsCong : forall (psi:grade) (g1 g3 g4:co),
      (lc_co g1) ->
       ( forall c , lc_co  ( open_co_wrt_co g3 (g_Var_f c) )  )  ->
      (lc_co g4) ->
-     (lc_co (g_CAbsCong g1 g3 g4))
+     (lc_co (g_CAbsCong psi g1 g3 g4))
  | lc_g_CAppCong : forall (g g1 g2:co),
      (lc_co g) ->
      (lc_co g1) ->
@@ -368,46 +368,44 @@ with lc_tm : tm -> Prop :=    (* defn lc_tm *)
      (lc_tm a_Star)
  | lc_a_Var_f : forall (x:tmvar),
      (lc_tm (a_Var_f x))
- | lc_a_Abs : forall (rho:relflag) (A b:tm),
+ | lc_a_Abs : forall (psi:grade) (A b:tm),
      (lc_tm A) ->
       ( forall x , lc_tm  ( open_tm_wrt_tm b (a_Var_f x) )  )  ->
-     (lc_tm (a_Abs rho A b))
- | lc_a_UAbs : forall (rho:relflag) (b:tm),
+     (lc_tm (a_Abs psi A b))
+ | lc_a_UAbs : forall (psi:grade) (b:tm),
       ( forall x , lc_tm  ( open_tm_wrt_tm b (a_Var_f x) )  )  ->
-     (lc_tm (a_UAbs rho b))
- | lc_a_App : forall (a:tm) (rho:relflag) (b:tm),
+     (lc_tm (a_UAbs psi b))
+ | lc_a_App : forall (a:tm) (psi:grade) (b:tm),
      (lc_tm a) ->
      (lc_tm b) ->
-     (lc_tm (a_App a rho b))
+     (lc_tm (a_App a psi b))
  | lc_a_Fam : forall (F:tyfam),
      (lc_tm (a_Fam F))
  | lc_a_Const : forall (T:const),
      (lc_tm (a_Const T))
- | lc_a_Pi : forall (rho:relflag) (A B:tm),
+ | lc_a_Pi : forall (psi:grade) (A B:tm),
      (lc_tm A) ->
       ( forall x , lc_tm  ( open_tm_wrt_tm B (a_Var_f x) )  )  ->
-     (lc_tm (a_Pi rho A B))
+     (lc_tm (a_Pi psi A B))
  | lc_a_Conv : forall (a:tm) (g:co),
      (lc_tm a) ->
      (lc_co g) ->
      (lc_tm (a_Conv a g))
- | lc_a_CPi : forall (phi:constraint) (B:tm),
+ | lc_a_CPi : forall (psi:grade) (phi:constraint) (B:tm),
      (lc_constraint phi) ->
       ( forall c , lc_tm  ( open_tm_wrt_co B (g_Var_f c) )  )  ->
-     (lc_tm (a_CPi phi B))
- | lc_a_CAbs : forall (phi:constraint) (b:tm),
+     (lc_tm (a_CPi psi phi B))
+ | lc_a_CAbs : forall (psi:grade) (phi:constraint) (b:tm),
      (lc_constraint phi) ->
       ( forall c , lc_tm  ( open_tm_wrt_co b (g_Var_f c) )  )  ->
-     (lc_tm (a_CAbs phi b))
- | lc_a_UCAbs : forall (b:tm),
+     (lc_tm (a_CAbs psi phi b))
+ | lc_a_UCAbs : forall (psi:grade) (b:tm),
       ( forall c , lc_tm  ( open_tm_wrt_co b (g_Var_f c) )  )  ->
-     (lc_tm (a_UCAbs b))
+     (lc_tm (a_UCAbs psi b))
  | lc_a_CApp : forall (a:tm) (g:co),
      (lc_tm a) ->
      (lc_co g) ->
      (lc_tm (a_CApp a g))
- | lc_a_Bullet : 
-     (lc_tm a_Bullet)
  | lc_a_DataCon : forall (K:datacon),
      (lc_tm (a_DataCon K))
  | lc_a_Case : forall (a:tm) (brs5:brs),
@@ -425,15 +423,6 @@ with lc_constraint : constraint -> Prop :=    (* defn lc_constraint *)
      (lc_constraint phi2) ->
      (lc_constraint (Impl phi1 phi2)).
 
-(* defns LC_sort *)
-Inductive lc_sort : sort -> Prop :=    (* defn lc_sort *)
- | lc_Tm : forall (A:tm),
-     (lc_tm A) ->
-     (lc_sort (Tm A))
- | lc_Co : forall (phi:constraint),
-     (lc_constraint phi) ->
-     (lc_sort (Co phi)).
-
 (* defns LC_sig_sort *)
 Inductive lc_sig_sort : sig_sort -> Prop :=    (* defn lc_sig_sort *)
  | lc_Cs : forall (A:tm),
@@ -443,6 +432,15 @@ Inductive lc_sig_sort : sig_sort -> Prop :=    (* defn lc_sig_sort *)
      (lc_tm a) ->
      (lc_tm A) ->
      (lc_sig_sort (Ax a A)).
+
+(* defns LC_sort *)
+Inductive lc_sort : sort -> Prop :=    (* defn lc_sort *)
+ | lc_Tm : forall (A:tm),
+     (lc_tm A) ->
+     (lc_sort (Tm A))
+ | lc_Co : forall (phi:constraint),
+     (lc_constraint phi) ->
+     (lc_sort (Co phi)).
 (** free variables *)
 Fixpoint fv_tm_tm_co (g_5:co) : vars :=
   match g_5 with
@@ -454,15 +452,15 @@ Fixpoint fv_tm_tm_co (g_5:co) : vars :=
   | (g_Refl2 a b g) => (fv_tm_tm_tm a) \u (fv_tm_tm_tm b) \u (fv_tm_tm_co g)
   | (g_Sym g) => (fv_tm_tm_co g)
   | (g_Trans g1 g2) => (fv_tm_tm_co g1) \u (fv_tm_tm_co g2)
-  | (g_PiCong rho g1 g2) => (fv_tm_tm_co g1) \u (fv_tm_tm_co g2)
-  | (g_AbsCong rho g1 g2) => (fv_tm_tm_co g1) \u (fv_tm_tm_co g2)
-  | (g_AppCong g1 rho g2) => (fv_tm_tm_co g1) \u (fv_tm_tm_co g2)
+  | (g_PiCong psi g1 g2) => (fv_tm_tm_co g1) \u (fv_tm_tm_co g2)
+  | (g_AbsCong psi g1 g2) => (fv_tm_tm_co g1) \u (fv_tm_tm_co g2)
+  | (g_AppCong g1 psi g2) => (fv_tm_tm_co g1) \u (fv_tm_tm_co g2)
   | (g_PiFst g) => (fv_tm_tm_co g)
   | (g_CPiFst g) => (fv_tm_tm_co g)
   | (g_IsoSnd g) => (fv_tm_tm_co g)
   | (g_PiSnd g1 g2) => (fv_tm_tm_co g1) \u (fv_tm_tm_co g2)
   | (g_CPiCong g1 g3) => (fv_tm_tm_co g1) \u (fv_tm_tm_co g3)
-  | (g_CAbsCong g1 g3 g4) => (fv_tm_tm_co g1) \u (fv_tm_tm_co g3) \u (fv_tm_tm_co g4)
+  | (g_CAbsCong psi g1 g3 g4) => (fv_tm_tm_co g1) \u (fv_tm_tm_co g3) \u (fv_tm_tm_co g4)
   | (g_CAppCong g g1 g2) => (fv_tm_tm_co g) \u (fv_tm_tm_co g1) \u (fv_tm_tm_co g2)
   | (g_CPiSnd g g1 g2) => (fv_tm_tm_co g) \u (fv_tm_tm_co g1) \u (fv_tm_tm_co g2)
   | (g_Cast g1 g2) => (fv_tm_tm_co g1) \u (fv_tm_tm_co g2)
@@ -482,18 +480,17 @@ with fv_tm_tm_tm (a5:tm) : vars :=
   | a_Star => {}
   | (a_Var_b nat) => {}
   | (a_Var_f x) => {{x}}
-  | (a_Abs rho A b) => (fv_tm_tm_tm A) \u (fv_tm_tm_tm b)
-  | (a_UAbs rho b) => (fv_tm_tm_tm b)
-  | (a_App a rho b) => (fv_tm_tm_tm a) \u (fv_tm_tm_tm b)
+  | (a_Abs psi A b) => (fv_tm_tm_tm A) \u (fv_tm_tm_tm b)
+  | (a_UAbs psi b) => (fv_tm_tm_tm b)
+  | (a_App a psi b) => (fv_tm_tm_tm a) \u (fv_tm_tm_tm b)
   | (a_Fam F) => {}
   | (a_Const T) => {}
-  | (a_Pi rho A B) => (fv_tm_tm_tm A) \u (fv_tm_tm_tm B)
+  | (a_Pi psi A B) => (fv_tm_tm_tm A) \u (fv_tm_tm_tm B)
   | (a_Conv a g) => (fv_tm_tm_tm a) \u (fv_tm_tm_co g)
-  | (a_CPi phi B) => (fv_tm_tm_constraint phi) \u (fv_tm_tm_tm B)
-  | (a_CAbs phi b) => (fv_tm_tm_constraint phi) \u (fv_tm_tm_tm b)
-  | (a_UCAbs b) => (fv_tm_tm_tm b)
+  | (a_CPi psi phi B) => (fv_tm_tm_constraint phi) \u (fv_tm_tm_tm B)
+  | (a_CAbs psi phi b) => (fv_tm_tm_constraint phi) \u (fv_tm_tm_tm b)
+  | (a_UCAbs psi b) => (fv_tm_tm_tm b)
   | (a_CApp a g) => (fv_tm_tm_tm a) \u (fv_tm_tm_co g)
-  | a_Bullet => {}
   | (a_DataCon K) => {}
   | (a_Case a brs5) => (fv_tm_tm_tm a) \u (fv_tm_tm_brs brs5)
 end
@@ -513,15 +510,15 @@ Fixpoint fv_co_co_co (g_5:co) : vars :=
   | (g_Refl2 a b g) => (fv_co_co_tm a) \u (fv_co_co_tm b) \u (fv_co_co_co g)
   | (g_Sym g) => (fv_co_co_co g)
   | (g_Trans g1 g2) => (fv_co_co_co g1) \u (fv_co_co_co g2)
-  | (g_PiCong rho g1 g2) => (fv_co_co_co g1) \u (fv_co_co_co g2)
-  | (g_AbsCong rho g1 g2) => (fv_co_co_co g1) \u (fv_co_co_co g2)
-  | (g_AppCong g1 rho g2) => (fv_co_co_co g1) \u (fv_co_co_co g2)
+  | (g_PiCong psi g1 g2) => (fv_co_co_co g1) \u (fv_co_co_co g2)
+  | (g_AbsCong psi g1 g2) => (fv_co_co_co g1) \u (fv_co_co_co g2)
+  | (g_AppCong g1 psi g2) => (fv_co_co_co g1) \u (fv_co_co_co g2)
   | (g_PiFst g) => (fv_co_co_co g)
   | (g_CPiFst g) => (fv_co_co_co g)
   | (g_IsoSnd g) => (fv_co_co_co g)
   | (g_PiSnd g1 g2) => (fv_co_co_co g1) \u (fv_co_co_co g2)
   | (g_CPiCong g1 g3) => (fv_co_co_co g1) \u (fv_co_co_co g3)
-  | (g_CAbsCong g1 g3 g4) => (fv_co_co_co g1) \u (fv_co_co_co g3) \u (fv_co_co_co g4)
+  | (g_CAbsCong psi g1 g3 g4) => (fv_co_co_co g1) \u (fv_co_co_co g3) \u (fv_co_co_co g4)
   | (g_CAppCong g g1 g2) => (fv_co_co_co g) \u (fv_co_co_co g1) \u (fv_co_co_co g2)
   | (g_CPiSnd g g1 g2) => (fv_co_co_co g) \u (fv_co_co_co g1) \u (fv_co_co_co g2)
   | (g_Cast g1 g2) => (fv_co_co_co g1) \u (fv_co_co_co g2)
@@ -541,18 +538,17 @@ with fv_co_co_tm (a5:tm) : vars :=
   | a_Star => {}
   | (a_Var_b nat) => {}
   | (a_Var_f x) => {}
-  | (a_Abs rho A b) => (fv_co_co_tm A) \u (fv_co_co_tm b)
-  | (a_UAbs rho b) => (fv_co_co_tm b)
-  | (a_App a rho b) => (fv_co_co_tm a) \u (fv_co_co_tm b)
+  | (a_Abs psi A b) => (fv_co_co_tm A) \u (fv_co_co_tm b)
+  | (a_UAbs psi b) => (fv_co_co_tm b)
+  | (a_App a psi b) => (fv_co_co_tm a) \u (fv_co_co_tm b)
   | (a_Fam F) => {}
   | (a_Const T) => {}
-  | (a_Pi rho A B) => (fv_co_co_tm A) \u (fv_co_co_tm B)
+  | (a_Pi psi A B) => (fv_co_co_tm A) \u (fv_co_co_tm B)
   | (a_Conv a g) => (fv_co_co_tm a) \u (fv_co_co_co g)
-  | (a_CPi phi B) => (fv_co_co_constraint phi) \u (fv_co_co_tm B)
-  | (a_CAbs phi b) => (fv_co_co_constraint phi) \u (fv_co_co_tm b)
-  | (a_UCAbs b) => (fv_co_co_tm b)
+  | (a_CPi psi phi B) => (fv_co_co_constraint phi) \u (fv_co_co_tm B)
+  | (a_CAbs psi phi b) => (fv_co_co_constraint phi) \u (fv_co_co_tm b)
+  | (a_UCAbs psi b) => (fv_co_co_tm b)
   | (a_CApp a g) => (fv_co_co_tm a) \u (fv_co_co_co g)
-  | a_Bullet => {}
   | (a_DataCon K) => {}
   | (a_Case a brs5) => (fv_co_co_tm a) \u (fv_co_co_brs brs5)
 end
@@ -560,18 +556,6 @@ with fv_co_co_constraint (phi_5:constraint) : vars :=
   match phi_5 with
   | (Eq a b A) => (fv_co_co_tm a) \u (fv_co_co_tm b) \u (fv_co_co_tm A)
   | (Impl phi1 phi2) => (fv_co_co_constraint phi1) \u (fv_co_co_constraint phi2)
-end.
-
-Definition fv_tm_tm_sig_sort (sig_sort5:sig_sort) : vars :=
-  match sig_sort5 with
-  | (Cs A) => (fv_tm_tm_tm A)
-  | (Ax a A) => (fv_tm_tm_tm a) \u (fv_tm_tm_tm A)
-end.
-
-Definition fv_co_co_sig_sort (sig_sort5:sig_sort) : vars :=
-  match sig_sort5 with
-  | (Cs A) => (fv_co_co_tm A)
-  | (Ax a A) => (fv_co_co_tm a) \u (fv_co_co_tm A)
 end.
 
 Definition fv_tm_tm_sort (sort5:sort) : vars :=
@@ -586,6 +570,18 @@ Definition fv_co_co_sort (sort5:sort) : vars :=
   | (Co phi) => (fv_co_co_constraint phi)
 end.
 
+Definition fv_tm_tm_sig_sort (sig_sort5:sig_sort) : vars :=
+  match sig_sort5 with
+  | (Cs A) => (fv_tm_tm_tm A)
+  | (Ax a A) => (fv_tm_tm_tm a) \u (fv_tm_tm_tm A)
+end.
+
+Definition fv_co_co_sig_sort (sig_sort5:sig_sort) : vars :=
+  match sig_sort5 with
+  | (Cs A) => (fv_co_co_tm A)
+  | (Ax a A) => (fv_co_co_tm a) \u (fv_co_co_tm A)
+end.
+
 (** substitutions *)
 Fixpoint tm_subst_tm_co (a5:tm) (x5:tmvar) (g_5:co) {struct g_5} : co :=
   match g_5 with
@@ -597,15 +593,15 @@ Fixpoint tm_subst_tm_co (a5:tm) (x5:tmvar) (g_5:co) {struct g_5} : co :=
   | (g_Refl2 a b g) => g_Refl2 (tm_subst_tm_tm a5 x5 a) (tm_subst_tm_tm a5 x5 b) (tm_subst_tm_co a5 x5 g)
   | (g_Sym g) => g_Sym (tm_subst_tm_co a5 x5 g)
   | (g_Trans g1 g2) => g_Trans (tm_subst_tm_co a5 x5 g1) (tm_subst_tm_co a5 x5 g2)
-  | (g_PiCong rho g1 g2) => g_PiCong rho (tm_subst_tm_co a5 x5 g1) (tm_subst_tm_co a5 x5 g2)
-  | (g_AbsCong rho g1 g2) => g_AbsCong rho (tm_subst_tm_co a5 x5 g1) (tm_subst_tm_co a5 x5 g2)
-  | (g_AppCong g1 rho g2) => g_AppCong (tm_subst_tm_co a5 x5 g1) rho (tm_subst_tm_co a5 x5 g2)
+  | (g_PiCong psi g1 g2) => g_PiCong psi (tm_subst_tm_co a5 x5 g1) (tm_subst_tm_co a5 x5 g2)
+  | (g_AbsCong psi g1 g2) => g_AbsCong psi (tm_subst_tm_co a5 x5 g1) (tm_subst_tm_co a5 x5 g2)
+  | (g_AppCong g1 psi g2) => g_AppCong (tm_subst_tm_co a5 x5 g1) psi (tm_subst_tm_co a5 x5 g2)
   | (g_PiFst g) => g_PiFst (tm_subst_tm_co a5 x5 g)
   | (g_CPiFst g) => g_CPiFst (tm_subst_tm_co a5 x5 g)
   | (g_IsoSnd g) => g_IsoSnd (tm_subst_tm_co a5 x5 g)
   | (g_PiSnd g1 g2) => g_PiSnd (tm_subst_tm_co a5 x5 g1) (tm_subst_tm_co a5 x5 g2)
   | (g_CPiCong g1 g3) => g_CPiCong (tm_subst_tm_co a5 x5 g1) (tm_subst_tm_co a5 x5 g3)
-  | (g_CAbsCong g1 g3 g4) => g_CAbsCong (tm_subst_tm_co a5 x5 g1) (tm_subst_tm_co a5 x5 g3) (tm_subst_tm_co a5 x5 g4)
+  | (g_CAbsCong psi g1 g3 g4) => g_CAbsCong psi (tm_subst_tm_co a5 x5 g1) (tm_subst_tm_co a5 x5 g3) (tm_subst_tm_co a5 x5 g4)
   | (g_CAppCong g g1 g2) => g_CAppCong (tm_subst_tm_co a5 x5 g) (tm_subst_tm_co a5 x5 g1) (tm_subst_tm_co a5 x5 g2)
   | (g_CPiSnd g g1 g2) => g_CPiSnd (tm_subst_tm_co a5 x5 g) (tm_subst_tm_co a5 x5 g1) (tm_subst_tm_co a5 x5 g2)
   | (g_Cast g1 g2) => g_Cast (tm_subst_tm_co a5 x5 g1) (tm_subst_tm_co a5 x5 g2)
@@ -625,18 +621,17 @@ with tm_subst_tm_tm (a5:tm) (x5:tmvar) (a_6:tm) {struct a_6} : tm :=
   | a_Star => a_Star 
   | (a_Var_b nat) => a_Var_b nat
   | (a_Var_f x) => (if eq_var x x5 then a5 else (a_Var_f x))
-  | (a_Abs rho A b) => a_Abs rho (tm_subst_tm_tm a5 x5 A) (tm_subst_tm_tm a5 x5 b)
-  | (a_UAbs rho b) => a_UAbs rho (tm_subst_tm_tm a5 x5 b)
-  | (a_App a rho b) => a_App (tm_subst_tm_tm a5 x5 a) rho (tm_subst_tm_tm a5 x5 b)
+  | (a_Abs psi A b) => a_Abs psi (tm_subst_tm_tm a5 x5 A) (tm_subst_tm_tm a5 x5 b)
+  | (a_UAbs psi b) => a_UAbs psi (tm_subst_tm_tm a5 x5 b)
+  | (a_App a psi b) => a_App (tm_subst_tm_tm a5 x5 a) psi (tm_subst_tm_tm a5 x5 b)
   | (a_Fam F) => a_Fam F
   | (a_Const T) => a_Const T
-  | (a_Pi rho A B) => a_Pi rho (tm_subst_tm_tm a5 x5 A) (tm_subst_tm_tm a5 x5 B)
+  | (a_Pi psi A B) => a_Pi psi (tm_subst_tm_tm a5 x5 A) (tm_subst_tm_tm a5 x5 B)
   | (a_Conv a g) => a_Conv (tm_subst_tm_tm a5 x5 a) (tm_subst_tm_co a5 x5 g)
-  | (a_CPi phi B) => a_CPi (tm_subst_tm_constraint a5 x5 phi) (tm_subst_tm_tm a5 x5 B)
-  | (a_CAbs phi b) => a_CAbs (tm_subst_tm_constraint a5 x5 phi) (tm_subst_tm_tm a5 x5 b)
-  | (a_UCAbs b) => a_UCAbs (tm_subst_tm_tm a5 x5 b)
+  | (a_CPi psi phi B) => a_CPi psi (tm_subst_tm_constraint a5 x5 phi) (tm_subst_tm_tm a5 x5 B)
+  | (a_CAbs psi phi b) => a_CAbs psi (tm_subst_tm_constraint a5 x5 phi) (tm_subst_tm_tm a5 x5 b)
+  | (a_UCAbs psi b) => a_UCAbs psi (tm_subst_tm_tm a5 x5 b)
   | (a_CApp a g) => a_CApp (tm_subst_tm_tm a5 x5 a) (tm_subst_tm_co a5 x5 g)
-  | a_Bullet => a_Bullet 
   | (a_DataCon K) => a_DataCon K
   | (a_Case a brs5) => a_Case (tm_subst_tm_tm a5 x5 a) (tm_subst_tm_brs a5 x5 brs5)
 end
@@ -656,15 +651,15 @@ Fixpoint co_subst_co_co (g_5:co) (c5:covar) (g__6:co) {struct g__6} : co :=
   | (g_Refl2 a b g) => g_Refl2 (co_subst_co_tm g_5 c5 a) (co_subst_co_tm g_5 c5 b) (co_subst_co_co g_5 c5 g)
   | (g_Sym g) => g_Sym (co_subst_co_co g_5 c5 g)
   | (g_Trans g1 g2) => g_Trans (co_subst_co_co g_5 c5 g1) (co_subst_co_co g_5 c5 g2)
-  | (g_PiCong rho g1 g2) => g_PiCong rho (co_subst_co_co g_5 c5 g1) (co_subst_co_co g_5 c5 g2)
-  | (g_AbsCong rho g1 g2) => g_AbsCong rho (co_subst_co_co g_5 c5 g1) (co_subst_co_co g_5 c5 g2)
-  | (g_AppCong g1 rho g2) => g_AppCong (co_subst_co_co g_5 c5 g1) rho (co_subst_co_co g_5 c5 g2)
+  | (g_PiCong psi g1 g2) => g_PiCong psi (co_subst_co_co g_5 c5 g1) (co_subst_co_co g_5 c5 g2)
+  | (g_AbsCong psi g1 g2) => g_AbsCong psi (co_subst_co_co g_5 c5 g1) (co_subst_co_co g_5 c5 g2)
+  | (g_AppCong g1 psi g2) => g_AppCong (co_subst_co_co g_5 c5 g1) psi (co_subst_co_co g_5 c5 g2)
   | (g_PiFst g) => g_PiFst (co_subst_co_co g_5 c5 g)
   | (g_CPiFst g) => g_CPiFst (co_subst_co_co g_5 c5 g)
   | (g_IsoSnd g) => g_IsoSnd (co_subst_co_co g_5 c5 g)
   | (g_PiSnd g1 g2) => g_PiSnd (co_subst_co_co g_5 c5 g1) (co_subst_co_co g_5 c5 g2)
   | (g_CPiCong g1 g3) => g_CPiCong (co_subst_co_co g_5 c5 g1) (co_subst_co_co g_5 c5 g3)
-  | (g_CAbsCong g1 g3 g4) => g_CAbsCong (co_subst_co_co g_5 c5 g1) (co_subst_co_co g_5 c5 g3) (co_subst_co_co g_5 c5 g4)
+  | (g_CAbsCong psi g1 g3 g4) => g_CAbsCong psi (co_subst_co_co g_5 c5 g1) (co_subst_co_co g_5 c5 g3) (co_subst_co_co g_5 c5 g4)
   | (g_CAppCong g g1 g2) => g_CAppCong (co_subst_co_co g_5 c5 g) (co_subst_co_co g_5 c5 g1) (co_subst_co_co g_5 c5 g2)
   | (g_CPiSnd g g1 g2) => g_CPiSnd (co_subst_co_co g_5 c5 g) (co_subst_co_co g_5 c5 g1) (co_subst_co_co g_5 c5 g2)
   | (g_Cast g1 g2) => g_Cast (co_subst_co_co g_5 c5 g1) (co_subst_co_co g_5 c5 g2)
@@ -684,18 +679,17 @@ with co_subst_co_tm (g5:co) (c5:covar) (a5:tm) {struct a5} : tm :=
   | a_Star => a_Star 
   | (a_Var_b nat) => a_Var_b nat
   | (a_Var_f x) => a_Var_f x
-  | (a_Abs rho A b) => a_Abs rho (co_subst_co_tm g5 c5 A) (co_subst_co_tm g5 c5 b)
-  | (a_UAbs rho b) => a_UAbs rho (co_subst_co_tm g5 c5 b)
-  | (a_App a rho b) => a_App (co_subst_co_tm g5 c5 a) rho (co_subst_co_tm g5 c5 b)
+  | (a_Abs psi A b) => a_Abs psi (co_subst_co_tm g5 c5 A) (co_subst_co_tm g5 c5 b)
+  | (a_UAbs psi b) => a_UAbs psi (co_subst_co_tm g5 c5 b)
+  | (a_App a psi b) => a_App (co_subst_co_tm g5 c5 a) psi (co_subst_co_tm g5 c5 b)
   | (a_Fam F) => a_Fam F
   | (a_Const T) => a_Const T
-  | (a_Pi rho A B) => a_Pi rho (co_subst_co_tm g5 c5 A) (co_subst_co_tm g5 c5 B)
+  | (a_Pi psi A B) => a_Pi psi (co_subst_co_tm g5 c5 A) (co_subst_co_tm g5 c5 B)
   | (a_Conv a g) => a_Conv (co_subst_co_tm g5 c5 a) (co_subst_co_co g5 c5 g)
-  | (a_CPi phi B) => a_CPi (co_subst_co_constraint g5 c5 phi) (co_subst_co_tm g5 c5 B)
-  | (a_CAbs phi b) => a_CAbs (co_subst_co_constraint g5 c5 phi) (co_subst_co_tm g5 c5 b)
-  | (a_UCAbs b) => a_UCAbs (co_subst_co_tm g5 c5 b)
+  | (a_CPi psi phi B) => a_CPi psi (co_subst_co_constraint g5 c5 phi) (co_subst_co_tm g5 c5 B)
+  | (a_CAbs psi phi b) => a_CAbs psi (co_subst_co_constraint g5 c5 phi) (co_subst_co_tm g5 c5 b)
+  | (a_UCAbs psi b) => a_UCAbs psi (co_subst_co_tm g5 c5 b)
   | (a_CApp a g) => a_CApp (co_subst_co_tm g5 c5 a) (co_subst_co_co g5 c5 g)
-  | a_Bullet => a_Bullet 
   | (a_DataCon K) => a_DataCon K
   | (a_Case a brs5) => a_Case (co_subst_co_tm g5 c5 a) (co_subst_co_brs g5 c5 brs5)
 end
@@ -729,6 +723,23 @@ Definition co_subst_co_sig_sort (g5:co) (c5:covar) (sig_sort5:sig_sort) : sig_so
   | (Ax a A) => Ax (co_subst_co_tm g5 c5 a) (co_subst_co_tm g5 c5 A)
 end.
 
+Local Open Scope grade_scope.
+
+Definition labels : context -> econtext :=
+  map (fun '(u , s) => u).
+
+Definition join_ctx_l (psi : grade) : context -> context :=    
+  map (fun '(g, A) => (psi * g, A)).
+
+Definition join_ctx_r (psi : grade) : context -> context :=
+  map (fun '(g, A) => (g * psi, A)).
+
+Definition meet_ctx_l (psi : grade) : context -> context :=
+  map (fun '(g, A) => (psi + g, A)).
+
+Definition meet_ctx_r (psi : grade) : context -> context :=
+  map (fun '(g, A) => (g + psi, A)).
+
 Fixpoint erase_tm (a : tm) : tm :=
    match a with
    | a_Star    => a_Star
@@ -736,19 +747,17 @@ Fixpoint erase_tm (a : tm) : tm :=
    | a_Var_f x => a_Var_f x
    | a_Abs rho A b => a_UAbs rho (erase_tm b)
    | a_UAbs rho b => a_UAbs rho (erase_tm b)
-   | a_App a Rel b => a_App (erase_tm a) Rel (erase_tm b)
-   | a_App a Irrel b => a_App (erase_tm a) Irrel a_Bullet
+   | a_App a psi0 b => a_App (erase_tm a) psi0 (erase_tm b)
    | a_Const T => a_Const T
    | a_Fam F => a_Fam F
    | a_Pi rho A B => a_Pi rho (erase_tm A) (erase_tm B)
    | a_Conv a _ => erase_tm a
-   | a_CPi phi B => a_CPi (erase_constraint phi) (erase_tm B)
-   | a_CAbs phi b => a_UCAbs (erase_tm b)
-   | a_UCAbs b => a_UCAbs (erase_tm b)
+   | a_CPi psi0 phi B => a_CPi psi0 (erase_constraint phi) (erase_tm B)
+   | a_CAbs psi0 phi b => a_UCAbs psi0 (erase_tm b)
+   | a_UCAbs psi0 b => a_UCAbs psi0 (erase_tm b)
    | a_CApp a g => a_CApp (erase_tm a) g_Triv
    | a_DataCon K => a_Star  (* a_DataCon K *)
    | a_Case a brs => a_Star (* a_Case (erase_tm a) (erase_brs brs) *)
-   | a_Bullet => a_Bullet
    end
 with erase_brs (x : brs) : brs :=
    match x with
@@ -774,7 +783,7 @@ Definition erase_csort s :=
  | Ax a A => Ax (erase_tm a) (erase_tm A)
 end.
 
-Definition erase_context G := map erase_sort G.
+Definition erase_context (G : context) := map (fun '(psi, s) => (psi, erase_sort s)) G.
 Definition erase_sig S := map erase_csort S.
 
 (* -------------- A specific signature with Fix ------------ *)
@@ -784,14 +793,14 @@ Definition Fix : atom.
 Qed.
 
 Definition FixDef : tm :=
-  (a_Abs Irrel a_Star
-         (a_Abs Rel (a_Pi Rel (a_Var_b 0) (a_Var_b 1))
-                (a_App (a_Var_b 0) Rel
-                       (a_App (a_App (a_Fam Fix) Irrel (a_Var_b 1)) Rel (a_Var_b 0))))).
+  (a_Abs q_C a_Star
+         (a_Abs q_R (a_Pi q_R (a_Var_b 0) (a_Var_b 1))
+                (a_App (a_Var_b 0) q_R
+                       (a_App (a_App (a_Fam Fix) q_C (a_Var_b 1)) q_R (a_Var_b 0))))).
 
 Definition FixTy : tm :=
-  a_Pi Irrel a_Star
-       (a_Pi Rel (a_Pi Rel (a_Var_b 0) (a_Var_b 1))
+  a_Pi q_C a_Star
+       (a_Pi q_R (a_Pi q_R (a_Var_b 0) (a_Var_b 1))
              (a_Var_b 1)).
 
 
@@ -815,63 +824,56 @@ Inductive CoercedValue : tm -> Prop :=    (* defn CoercedValue *)
 with Value : tm -> Prop :=    (* defn Value *)
  | Value_Star : 
      Value a_Star
- | Value_Pi : forall (rho:relflag) (A B:tm),
+ | Value_Pi : forall (psi:grade) (A B:tm),
      lc_tm A ->
-     lc_tm (a_Pi rho A B) ->
-     Value (a_Pi rho A B)
- | Value_CPi : forall (phi:constraint) (B:tm),
+     lc_tm (a_Pi psi A B) ->
+     Value (a_Pi psi A B)
+ | Value_CPi : forall (psi:grade) (phi:constraint) (B:tm),
      lc_constraint phi ->
-     lc_tm (a_CPi phi B) ->
-     Value (a_CPi phi B)
- | Value_AbsRel : forall (A a:tm),
+     lc_tm (a_CPi psi phi B) ->
+     Value (a_CPi psi phi B)
+ | Value_Abs : forall (psi:grade) (A a:tm),
      lc_tm A ->
-     lc_tm (a_Abs Rel A a) ->
-     Value (a_Abs Rel A a)
- | Value_UAbsRel : forall (a:tm),
-     lc_tm (a_UAbs Rel a) ->
-     Value (a_UAbs Rel a)
- | Value_UAbsIrrel : forall (L:vars) (a:tm),
-      ( forall x , x \notin  L  -> Value  ( open_tm_wrt_tm a (a_Var_f x) )  )  ->
-     Value (a_UAbs Irrel a)
- | Value_AbsIrrel : forall (L:vars) (A a:tm),
-     lc_tm A ->
-      ( forall x , x \notin  L  -> CoercedValue  ( open_tm_wrt_tm a (a_Var_f x) )  )  ->
-     Value (a_Abs Irrel A a)
- | Value_CAbs : forall (phi:constraint) (a:tm),
+     lc_tm (a_Abs psi A a) ->
+     Value (a_Abs psi A a)
+ | Value_UAbs : forall (psi:grade) (a:tm),
+     lc_tm (a_UAbs psi a) ->
+     Value (a_UAbs psi a)
+ | Value_CAbs : forall (psi:grade) (phi:constraint) (a:tm),
      lc_constraint phi ->
-     lc_tm (a_CAbs phi a) ->
-     Value (a_CAbs phi a)
- | Value_UCAbs : forall (a:tm),
-     lc_tm (a_UCAbs a) ->
-     Value (a_UCAbs a)
+     lc_tm (a_CAbs psi phi a) ->
+     Value (a_CAbs psi phi a)
+ | Value_UCAbs : forall (psi:grade) (a:tm),
+     lc_tm (a_UCAbs psi a) ->
+     Value (a_UCAbs psi a)
 with value_type : tm -> Prop :=    (* defn value_type *)
  | value_type_Star : 
      value_type a_Star
- | value_type_Pi : forall (rho:relflag) (A B:tm),
+ | value_type_Pi : forall (psi:grade) (A B:tm),
      lc_tm A ->
-     lc_tm (a_Pi rho A B) ->
-     value_type (a_Pi rho A B)
- | value_type_CPi : forall (phi:constraint) (B:tm),
+     lc_tm (a_Pi psi A B) ->
+     value_type (a_Pi psi A B)
+ | value_type_CPi : forall (psi:grade) (phi:constraint) (B:tm),
      lc_constraint phi ->
-     lc_tm (a_CPi phi B) ->
-     value_type (a_CPi phi B).
+     lc_tm (a_CPi psi phi B) ->
+     value_type (a_CPi psi phi B).
 
 (* defns Jconsistent *)
 Inductive consistent : tm -> tm -> Prop :=    (* defn consistent *)
  | consistent_a_Star : 
      consistent a_Star a_Star
- | consistent_a_Pi : forall (rho:relflag) (A1 B1 A2 B2:tm),
+ | consistent_a_Pi : forall (psi1:grade) (A1 B1:tm) (psi2:grade) (A2 B2:tm),
      lc_tm A1 ->
-     lc_tm (a_Pi rho A1 B1) ->
+     lc_tm (a_Pi psi1 A1 B1) ->
      lc_tm A2 ->
-     lc_tm (a_Pi rho A2 B2) ->
-     consistent  ( (a_Pi rho A1 B1) )   ( (a_Pi rho A2 B2) ) 
- | consistent_a_CPi : forall (phi1:constraint) (A1:tm) (phi2:constraint) (A2:tm),
+     lc_tm (a_Pi psi2 A2 B2) ->
+     consistent  ( (a_Pi psi1 A1 B1) )   ( (a_Pi psi2 A2 B2) ) 
+ | consistent_a_CPi : forall (psi1:grade) (phi1:constraint) (A1:tm) (psi2:grade) (phi2:constraint) (A2:tm),
      lc_constraint phi1 ->
-     lc_tm (a_CPi phi1 A1) ->
+     lc_tm (a_CPi psi1 phi1 A1) ->
      lc_constraint phi2 ->
-     lc_tm (a_CPi phi2 A2) ->
-     consistent  ( (a_CPi phi1 A1) )   ( (a_CPi phi2 A2) ) 
+     lc_tm (a_CPi psi2 phi2 A2) ->
+     consistent  ( (a_CPi psi1 phi1 A1) )   ( (a_CPi psi2 phi2 A2) ) 
  | consistent_a_Step_R : forall (a b:tm),
      lc_tm a ->
       not ( value_type b )  ->
@@ -880,15 +882,6 @@ Inductive consistent : tm -> tm -> Prop :=    (* defn consistent *)
      lc_tm b ->
       not ( value_type a )  ->
      consistent a b.
-
-(* defns JChk *)
-Inductive RhoCheck : relflag -> tmvar -> tm -> Prop :=    (* defn RhoCheck *)
- | Rho_Rel : forall (x:tmvar) (A:tm),
-      True  ->
-     RhoCheck Rel x A
- | Rho_IrrRel : forall (x:tmvar) (A:tm),
-      x  \notin fv_tm_tm_tm  A  ->
-     RhoCheck Irrel x A.
 
 (* defns Jerased *)
 Inductive erased_constraint : constraint -> Prop :=    (* defn erased_constraint *)
@@ -902,162 +895,291 @@ Inductive erased_constraint : constraint -> Prop :=    (* defn erased_constraint
      erased_constraint phi2 ->
      erased_constraint (Impl phi1 phi2)
 with erased_tm : tm -> Prop :=    (* defn erased_tm *)
- | erased_a_Bullet : 
-     erased_tm a_Bullet
  | erased_a_Star : 
      erased_tm a_Star
  | erased_a_Var : forall (x:tmvar),
      erased_tm (a_Var_f x)
- | erased_a_Abs : forall (L:vars) (rho:relflag) (a:tm),
+ | erased_a_Abs : forall (L:vars) (psi:grade) (a:tm),
       ( forall x , x \notin  L  -> erased_tm  ( open_tm_wrt_tm a (a_Var_f x) )  )  ->
-      ( forall x , x \notin  L  -> RhoCheck rho x  ( open_tm_wrt_tm a (a_Var_f x) )  )  ->
-     erased_tm  ( (a_UAbs rho a) ) 
- | erased_a_App : forall (a b:tm),
+     erased_tm  ( (a_UAbs psi a) ) 
+ | erased_a_App : forall (a:tm) (psi:grade) (b:tm),
      erased_tm a ->
      erased_tm b ->
-     erased_tm  ( (a_App a Rel b) ) 
- | erased_a_AppIrrel : forall (a:tm),
-     erased_tm a ->
-     erased_tm  ( (a_App a Irrel a_Bullet) ) 
- | erased_a_Pi : forall (L:vars) (rho:relflag) (A B:tm),
+     erased_tm  ( (a_App a psi b) ) 
+ | erased_a_Pi : forall (L:vars) (psi:grade) (A B:tm),
      erased_tm A ->
       ( forall x , x \notin  L  -> erased_tm  ( open_tm_wrt_tm B (a_Var_f x) )  )  ->
-     erased_tm  ( (a_Pi rho A B) ) 
- | erased_a_CPi : forall (L:vars) (phi:constraint) (B:tm),
+     erased_tm  ( (a_Pi psi A B) ) 
+ | erased_a_CPi : forall (L:vars) (psi:grade) (phi:constraint) (B:tm),
      erased_constraint phi ->
       ( forall c , c \notin  L  -> erased_tm  ( open_tm_wrt_co B (g_Var_f c) )  )  ->
-     erased_tm  ( (a_CPi phi B) ) 
- | erased_a_CAbs : forall (L:vars) (b:tm),
+     erased_tm  ( (a_CPi psi phi B) ) 
+ | erased_a_CAbs : forall (L:vars) (psi:grade) (b:tm),
       ( forall c , c \notin  L  -> erased_tm  ( open_tm_wrt_co b (g_Var_f c) )  )  ->
-     erased_tm  ( (a_UCAbs b) ) 
+     erased_tm  ( (a_UCAbs psi b) ) 
  | erased_a_CApp : forall (a:tm),
      erased_tm a ->
      erased_tm  ( (a_CApp a g_Triv) ) 
  | erased_a_Fam : forall (F:tyfam),
      erased_tm (a_Fam F).
 
-(* defns Jpar *)
-Inductive ParProp : context -> available_props -> constraint -> constraint -> Prop :=    (* defn ParProp *)
- | ParProp_Eq : forall (G:context) (D:available_props) (a b A a' b' A':tm),
-     Par G D a a' ->
-     Par G D b b' ->
-     Par G D A A' ->
-     ParProp G D (Eq a b A) (Eq a' b' A')
- | ParProp_Impl : forall (G:context) (D:available_props) (phi1 phi2 phi1' phi2':constraint),
-     ParProp G D phi1 phi1' ->
-     ParProp G D phi2 phi2' ->
-     ParProp G D (Impl phi1 phi2) (Impl phi1' phi2')
-with Par : context -> available_props -> tm -> tm -> Prop :=    (* defn Par *)
- | Par_Refl : forall (G:context) (D:available_props) (a:tm),
+(* defns Jsub *)
+Inductive P_sub : econtext -> econtext -> Prop :=    (* defn P_sub *)
+ | P_Empty : 
+     P_sub  nil   nil 
+ | P_Cons : forall (P1:econtext) (x:tmvar) (psi1:grade) (P2:econtext) (psi2:grade),
+      ( psi1  <=  psi2 )  ->
+     P_sub P1 P2 ->
+      ~ AtomSetImpl.In  x  (dom  P1 )  ->
+      ~ AtomSetImpl.In  x  (dom  P2 )  ->
+     P_sub  (( x ~  psi1 ) ++  P1 )   (( x ~  psi2 ) ++  P2 ) .
+
+(* defns Wsub *)
+Inductive ctx_sub : context -> context -> Prop :=    (* defn ctx_sub *)
+ | CS_Empty : 
+     ctx_sub  nil   nil 
+ | CS_ConsTm : forall (G1:context) (x:tmvar) (psi1:grade) (A:tm) (G2:context) (psi2:grade),
+      ( psi1  <=  psi2 )  ->
+     ctx_sub G1 G2 ->
+      ~ AtomSetImpl.In  x  (dom  G1 )  ->
+      ~ AtomSetImpl.In  x  (dom  G2 )  ->
+      True  ->
+     ctx_sub  (( x ~ ( psi1 , Tm  A )) ++  G1 )   (( x ~ ( psi2 , Tm  A )) ++  G2 ) 
+ | CS_ConsCo : forall (G1:context) (c:covar) (psi1:grade) (phi:constraint) (G2:context) (psi2:grade),
+     lc_constraint phi ->
+      ( psi1  <=  psi2 )  ->
+     ctx_sub G1 G2 ->
+      ~ AtomSetImpl.In  c  (dom  G1 )  ->
+      ~ AtomSetImpl.In  c  (dom  G2 )  ->
+     ctx_sub  (( c ~ ( psi1 , Co  phi )) ++  G1 )   (( c ~ ( psi2 , Co  phi )) ++  G2 ) .
+
+(* defns JGrade *)
+Inductive CoGrade : econtext -> grade -> constraint -> Prop :=    (* defn CoGrade *)
+ | CoG_Eq : forall (P:econtext) (psi:grade) (a b A:tm),
+     Grade P psi a ->
+     Grade P psi b ->
+     Grade P psi A ->
+     CoGrade P psi (Eq a b A)
+ | CoG_Impl : forall (P:econtext) (psi:grade) (phi1 phi2:constraint),
+     CoGrade P psi phi1 ->
+     CoGrade P psi phi2 ->
+     CoGrade P psi (Impl phi1 phi2)
+with CGrade : econtext -> grade -> grade -> tm -> Prop :=    (* defn CGrade *)
+ | CG_Leq : forall (P:econtext) (psi psi0:grade) (a:tm),
+      ( psi0  <=  psi )  ->
+     Grade P psi a ->
+     CGrade P psi psi0 a
+ | CG_Nleq : forall (P:econtext) (psi psi0:grade) (a:tm),
      lc_tm a ->
-     Par G D a a
- | Par_Beta : forall (G:context) (D:available_props) (a b a' b':tm),
-     Par G D a  ( (a_UAbs Rel a') )  ->
-     Par G D b b' ->
-     Par G D (a_App a Rel b)  (open_tm_wrt_tm  a'   b' ) 
- | Par_BetaIrrel : forall (G:context) (D:available_props) (a a':tm),
-     Par G D a  ( (a_UAbs Irrel a') )  ->
-     Par G D (a_App a Irrel a_Bullet)  (open_tm_wrt_tm  a'   a_Bullet ) 
- | Par_App : forall (G:context) (D:available_props) (a b a' b':tm),
-     Par G D a a' ->
-     Par G D b b' ->
-     Par G D (a_App a Rel b) (a_App a' Rel b')
- | Par_AppIrrel : forall (G:context) (D:available_props) (a a':tm),
-     Par G D a a' ->
-     Par G D (a_App a Irrel a_Bullet) (a_App a' Irrel a_Bullet)
- | Par_CBeta : forall (G:context) (D:available_props) (a a':tm),
-     Par G D a  ( (a_UCAbs a') )  ->
-     Par G D (a_CApp a g_Triv)  (open_tm_wrt_co  a'   g_Triv ) 
- | Par_CApp : forall (G:context) (D:available_props) (a a':tm),
-     Par G D a a' ->
-     Par G D (a_CApp a g_Triv) (a_CApp a' g_Triv)
- | Par_Abs : forall (L:vars) (G:context) (D:available_props) (rho:relflag) (a a':tm),
-      ( forall x , x \notin  L  -> Par G D  ( open_tm_wrt_tm a (a_Var_f x) )   ( open_tm_wrt_tm a' (a_Var_f x) )  )  ->
-     Par G D (a_UAbs rho a) (a_UAbs rho a')
- | Par_Pi : forall (L:vars) (G:context) (D:available_props) (rho:relflag) (A B A' B':tm),
-     Par G D A A' ->
-      ( forall x , x \notin  L  -> Par G D  ( open_tm_wrt_tm B (a_Var_f x) )   ( open_tm_wrt_tm B' (a_Var_f x) )  )  ->
-     Par G D (a_Pi rho A B) (a_Pi rho A' B')
- | Par_CAbs : forall (L:vars) (G:context) (D:available_props) (a a':tm),
-      ( forall c , c \notin  L  -> Par G D  ( open_tm_wrt_co a (g_Var_f c) )   ( open_tm_wrt_co a' (g_Var_f c) )  )  ->
-     Par G D (a_UCAbs a) (a_UCAbs a')
- | Par_CPi : forall (L:vars) (G:context) (D:available_props) (phi:constraint) (a:tm) (phi':constraint) (a':tm),
-      ( forall c , c \notin  L  -> Par G D  ( open_tm_wrt_co a (g_Var_f c) )   ( open_tm_wrt_co a' (g_Var_f c) )  )  ->
-     ParProp G D phi phi' ->
-     Par G D (a_CPi phi a) (a_CPi phi' a')
- | Par_Axiom : forall (G:context) (D:available_props) (F:tyfam) (a A:tm),
+      not (  (  ( psi0  <=  psi )  )  )  ->
+      uniq  P  ->
+     CGrade P psi psi0 a
+with Grade : econtext -> grade -> tm -> Prop :=    (* defn Grade *)
+ | G_Var : forall (P:econtext) (psi:grade) (x:tmvar) (psi0:grade),
+      uniq  P  ->
+      binds  x   psi0   P  ->
+      ( psi0  <=  psi )  ->
+     Grade P psi (a_Var_f x)
+ | G_Type : forall (P:econtext) (psi:grade),
+      uniq  P  ->
+     Grade P psi a_Star
+ | G_Pi : forall (L:vars) (P:econtext) (psi psi0:grade) (A B:tm),
+     Grade P psi A ->
+      ( forall x , x \notin  L  -> Grade  (( x ~  psi ) ++  P )  psi  ( open_tm_wrt_tm B (a_Var_f x) )  )  ->
+     Grade P psi (a_Pi psi0 A B)
+ | G_Abs : forall (L:vars) (P:econtext) (psi psi0:grade) (b:tm),
+      ( forall x , x \notin  L  -> Grade  (( x ~  psi0 ) ++  P )  psi  ( open_tm_wrt_tm b (a_Var_f x) )  )  ->
+     Grade P psi (a_UAbs psi0 b)
+ | G_App : forall (P:econtext) (psi:grade) (b:tm) (psi0:grade) (a:tm),
+     Grade P psi b ->
+     CGrade P psi psi0 a ->
+     Grade P psi (a_App b psi0 a)
+ | G_CPi : forall (L:vars) (P:econtext) (psi psi0:grade) (phi:constraint) (B:tm),
+     CoGrade P psi phi ->
+      ( forall c , c \notin  L  -> Grade  (( c ~  psi ) ++  P )  psi  ( open_tm_wrt_co B (g_Var_f c) )  )  ->
+     Grade P psi (a_CPi psi0 phi B)
+ | G_CAbs : forall (L:vars) (P:econtext) (psi psi0:grade) (b:tm),
+      ( forall c , c \notin  L  -> Grade  (( c ~  psi0 ) ++  P )  psi  ( open_tm_wrt_co b (g_Var_f c) )  )  ->
+     Grade P psi (a_UCAbs psi0 b)
+ | G_CApp : forall (P:econtext) (psi:grade) (b:tm),
+     Grade P psi b ->
+     Grade P psi (a_CApp b g_Triv).
+
+(* defns JGEq *)
+Inductive CoGEq : econtext -> grade -> constraint -> constraint -> Prop :=    (* defn CoGEq *)
+ | CoGEq_Eq : forall (P:econtext) (psi:grade) (a b A a' b' A':tm),
+     GEq P psi a a' ->
+     GEq P psi b b' ->
+     GEq P psi A A' ->
+     CoGEq P psi (Eq a b A) (Eq a' b' A')
+ | CoGEq_Impl : forall (P:econtext) (psi:grade) (phi1 phi3 phi2 phi4:constraint),
+     CoGEq P psi phi1 phi2 ->
+     CoGEq P psi phi3 phi4 ->
+     CoGEq P psi (Impl phi1 phi3) (Impl phi2 phi4)
+with CEq : econtext -> grade -> grade -> tm -> tm -> Prop :=    (* defn CEq *)
+ | CEq_Leq : forall (P:econtext) (psi psi0:grade) (a1 a2:tm),
+      ( psi0  <=  psi )  ->
+     GEq P psi a1 a2 ->
+     CEq P psi psi0 a1 a2
+ | CEq_Nleq : forall (P:econtext) (psi psi0:grade) (a1 a2:tm),
+     lc_tm a1 ->
+     lc_tm a2 ->
+      not (  (  ( psi0  <=  psi )  )  )  ->
+      uniq  P  ->
+     CEq P psi psi0 a1 a2
+with GEq : econtext -> grade -> tm -> tm -> Prop :=    (* defn GEq *)
+ | GEq_Var : forall (P:econtext) (psi:grade) (x:tmvar) (psi0:grade),
+      uniq  P  ->
+      binds  x   psi0   P  ->
+      ( psi0  <=  psi )  ->
+     GEq P psi (a_Var_f x) (a_Var_f x)
+ | GEq_Type : forall (P:econtext) (psi:grade),
+      uniq  P  ->
+     GEq P psi a_Star a_Star
+ | GEq_Pi : forall (L:vars) (P:econtext) (psi psi0:grade) (A1 B1 A2 B2:tm),
+     GEq P psi A1 A2 ->
+      ( forall x , x \notin  L  -> GEq  (( x ~  psi ) ++  P )  psi  ( open_tm_wrt_tm B1 (a_Var_f x) )   ( open_tm_wrt_tm B2 (a_Var_f x) )  )  ->
+     GEq P psi (a_Pi psi0 A1 B1) (a_Pi psi0 A2 B2)
+ | GEq_Abs : forall (L:vars) (P:econtext) (psi psi0:grade) (b1 b2:tm),
+      ( forall x , x \notin  L  -> GEq  (( x ~  psi0 ) ++  P )  psi  ( open_tm_wrt_tm b1 (a_Var_f x) )   ( open_tm_wrt_tm b2 (a_Var_f x) )  )  ->
+     GEq P psi (a_UAbs psi0 b1) (a_UAbs psi0 b2)
+ | GEq_App : forall (P:econtext) (psi:grade) (b1:tm) (psi0:grade) (a1 b2 a2:tm),
+     GEq P psi b1 b2 ->
+     CEq P psi psi0 a1 a2 ->
+     GEq P psi (a_App b1 psi0 a1) (a_App b2 psi0 a2)
+ | GEq_CPi : forall (L:vars) (P:econtext) (psi psi0:grade) (phi1:constraint) (B1:tm) (phi2:constraint) (B2:tm),
+     CoGEq P psi phi1 phi2 ->
+      ( forall c , c \notin  L  -> GEq  (( c ~  psi ) ++  P )  psi  ( open_tm_wrt_co B1 (g_Var_f c) )   ( open_tm_wrt_co B2 (g_Var_f c) )  )  ->
+     GEq P psi (a_CPi psi0 phi1 B1) (a_CPi psi0 phi2 B2)
+ | GEq_CAbs : forall (L:vars) (P:econtext) (psi psi0:grade) (b1 b2:tm),
+      ( forall c , c \notin  L  -> GEq  (( c ~  psi0 ) ++  P )  psi  ( open_tm_wrt_co b1 (g_Var_f c) )   ( open_tm_wrt_co b2 (g_Var_f c) )  )  ->
+     GEq P psi (a_UCAbs psi0 b1) (a_UCAbs psi0 b2)
+ | GEq_CApp : forall (P:econtext) (psi:grade) (b1 b2:tm),
+     GEq P psi b1 b2 ->
+     GEq P psi (a_CApp b1 g_Triv) (a_CApp b2 g_Triv).
+
+(* defns Jpar *)
+Inductive CParProp : econtext -> grade -> grade -> constraint -> constraint -> Prop :=    (* defn CParProp *)
+ | CParProp_Leq : forall (P:econtext) (psi psi0:grade) (phi1 phi2:constraint),
+      ( psi0  <=  psi )  ->
+     ParProp P psi phi1 phi2 ->
+     CParProp P psi psi0 phi1 phi2
+ | CParProp_Nleq : forall (P:econtext) (psi psi0:grade) (phi1 phi2:constraint),
+     lc_constraint phi1 ->
+     lc_constraint phi2 ->
+      not (  (  ( psi0  <=  psi )  )  )  ->
+      uniq  P  ->
+     CParProp P psi psi0 phi1 phi2
+with CPar : econtext -> grade -> grade -> tm -> tm -> Prop :=    (* defn CPar *)
+ | CPar_Leq : forall (P:econtext) (psi psi0:grade) (a1 a2:tm),
+      ( psi0  <=  psi )  ->
+     Par P psi a1 a2 ->
+     CPar P psi psi0 a1 a2
+ | CPar_Nleq : forall (P:econtext) (psi psi0:grade) (a1 a2:tm),
+     lc_tm a1 ->
+     lc_tm a2 ->
+      not (  (  ( psi0  <=  psi )  )  )  ->
+      uniq  P  ->
+     CPar P psi psi0 a1 a2
+with ParProp : econtext -> grade -> constraint -> constraint -> Prop :=    (* defn ParProp *)
+ | ParProp_Eq : forall (P:econtext) (psi:grade) (a b A a' b' A':tm),
+     Par P psi a a' ->
+     Par P psi b b' ->
+     Par P psi A A' ->
+     ParProp P psi (Eq a b A) (Eq a' b' A')
+ | ParProp_Impl : forall (P:econtext) (psi:grade) (phi1 phi2 phi1' phi2':constraint),
+     ParProp P psi phi1 phi1' ->
+     ParProp P psi phi2 phi2' ->
+     ParProp P psi (Impl phi1 phi2) (Impl phi1' phi2')
+with Par : econtext -> grade -> tm -> tm -> Prop :=    (* defn Par *)
+ | Par_Refl : forall (P:econtext) (psi:grade) (a:tm),
+     Grade P psi a ->
+     Par P psi a a
+ | Par_Beta : forall (P:econtext) (psi:grade) (a:tm) (psi0:grade) (b a' b':tm),
+     Par P psi a  ( (a_UAbs psi a') )  ->
+     CPar P psi psi0 b b' ->
+     Par P psi (a_App a psi0 b)  (open_tm_wrt_tm  a'   b' ) 
+ | Par_App : forall (P:econtext) (psi:grade) (a:tm) (psi0:grade) (b a' b':tm),
+     Par P psi a a' ->
+     CPar P psi psi0 b b' ->
+     Par P psi (a_App a psi0 b) (a_App a' psi0 b')
+ | Par_CBeta : forall (P:econtext) (psi:grade) (a a':tm) (psi0:grade),
+     Par P psi a  ( (a_UCAbs psi0 a') )  ->
+     Par P psi (a_CApp a g_Triv)  (open_tm_wrt_co  a'   g_Triv ) 
+ | Par_CApp : forall (P:econtext) (psi:grade) (a a':tm),
+     Par P psi a a' ->
+     Par P psi (a_CApp a g_Triv) (a_CApp a' g_Triv)
+ | Par_Abs : forall (L:vars) (P:econtext) (psi psi0:grade) (a a':tm),
+      ( forall x , x \notin  L  -> Par P psi  ( open_tm_wrt_tm a (a_Var_f x) )   ( open_tm_wrt_tm a' (a_Var_f x) )  )  ->
+     Par P psi (a_UAbs psi0 a) (a_UAbs psi0 a')
+ | Par_Pi : forall (L:vars) (P:econtext) (psi psi0:grade) (A B A' B':tm),
+     Par P psi A A' ->
+      ( forall x , x \notin  L  -> Par  (( x ~  psi ) ++  P )  psi  ( open_tm_wrt_tm B (a_Var_f x) )   ( open_tm_wrt_tm B' (a_Var_f x) )  )  ->
+     Par P psi (a_Pi psi0 A B) (a_Pi psi0 A' B')
+ | Par_CAbs : forall (L:vars) (P:econtext) (psi psi0:grade) (a a':tm),
+      ( forall c , c \notin  L  -> Par P psi  ( open_tm_wrt_co a (g_Var_f c) )   ( open_tm_wrt_co a' (g_Var_f c) )  )  ->
+     Par P psi (a_UCAbs psi0 a) (a_UCAbs psi0 a')
+ | Par_CPi : forall (L:vars) (P:econtext) (psi psi0:grade) (phi:constraint) (a:tm) (phi':constraint) (a':tm),
+      ( forall c , c \notin  L  -> Par  (( c ~  psi ) ++  P )  psi  ( open_tm_wrt_co a (g_Var_f c) )   ( open_tm_wrt_co a' (g_Var_f c) )  )  ->
+     ParProp P psi phi phi' ->
+     Par P psi (a_CPi psi0 phi a) (a_CPi psi0 phi' a')
+ | Par_Axiom : forall (P:econtext) (psi:grade) (F:tyfam) (a A:tm),
       binds  F  (Ax  a A )   toplevel   ->
-     Par G D (a_Fam F) a
- | Par_Eta : forall (L:vars) (G:context) (D:available_props) (a b' b:tm),
-     Par G D b b' ->
-      ( forall x , x \notin  L  ->  (  ( open_tm_wrt_tm a (a_Var_f x) )   =  (a_App b Rel (a_Var_f x)) )  )  ->
-     Par G D (a_UAbs Rel a) b'
- | Par_EtaIrrel : forall (L:vars) (G:context) (D:available_props) (a b' b:tm),
-     Par G D b b' ->
-      ( forall x , x \notin  L  ->  (  ( open_tm_wrt_tm a (a_Var_f x) )   =  (a_App b Irrel a_Bullet) )  )  ->
-     Par G D (a_UAbs Irrel a) b'
- | Par_EtaC : forall (L:vars) (G:context) (D:available_props) (a b' b:tm),
-     Par G D b b' ->
+     Par P psi (a_Fam F) a
+ | Par_Eta : forall (L:vars) (P:econtext) (psi psi0:grade) (a b' b:tm),
+     Par P psi b b' ->
+      ( forall x , x \notin  L  ->  (  ( open_tm_wrt_tm a (a_Var_f x) )   =  (a_App b psi0 (a_Var_f x)) )  )  ->
+     Par P psi (a_UAbs psi0 a) b'
+ | Par_EtaC : forall (L:vars) (P:econtext) (psi:grade) (a b' b:tm),
+     Par P psi b b' ->
       ( forall c , c \notin  L  ->  (  ( open_tm_wrt_co a (g_Var_f c) )   =  (a_CApp b g_Triv) )  )  ->
-     Par G D (a_UCAbs a) b'.
+     Par P psi (a_UCAbs  q_Top  a) b'.
 
 (* defns Jmultipar *)
-Inductive multipar : context -> available_props -> tm -> tm -> Prop :=    (* defn multipar *)
- | mp_refl : forall (G:context) (D:available_props) (a:tm),
+Inductive multipar : econtext -> grade -> tm -> tm -> Prop :=    (* defn multipar *)
+ | mp_refl : forall (P:econtext) (psi:grade) (a:tm),
      lc_tm a ->
-     multipar G D a a
- | mp_step : forall (G:context) (D:available_props) (a a' b:tm),
-     Par G D a b ->
-     multipar G D b a' ->
-     multipar G D a a'
-with multipar_prop : context -> available_props -> constraint -> constraint -> Prop :=    (* defn multipar_prop *)
- | mpprop_refl : forall (G:context) (D:available_props) (phi:constraint),
+     multipar P psi a a
+ | mp_step : forall (P:econtext) (psi:grade) (a a' b:tm),
+     Par P psi a b ->
+     multipar P psi b a' ->
+     multipar P psi a a'
+with multipar_prop : econtext -> grade -> constraint -> constraint -> Prop :=    (* defn multipar_prop *)
+ | mpprop_refl : forall (P:econtext) (psi:grade) (phi:constraint),
      lc_constraint phi ->
-     multipar_prop G D phi phi
- | mpprop_step : forall (G:context) (D:available_props) (phi1 phi3 phi2:constraint),
-     ParProp G D phi1 phi2 ->
-     multipar_prop G D phi2 phi3 ->
-     multipar_prop G D phi1 phi3.
+     multipar_prop P psi phi phi
+ | mpprop_step : forall (P:econtext) (psi:grade) (phi1 phi3 phi2:constraint),
+     ParProp P psi phi1 phi2 ->
+     multipar_prop P psi phi2 phi3 ->
+     multipar_prop P psi phi1 phi3.
 
 (* defns Jbeta *)
 Inductive Beta : tm -> tm -> Prop :=    (* defn Beta *)
- | Beta_AppAbs : forall (v b:tm),
-     lc_tm (a_UAbs Rel v) ->
+ | Beta_AppAbs : forall (psi:grade) (v b:tm),
+     lc_tm (a_UAbs psi v) ->
      lc_tm b ->
-     Beta (a_App  ( (a_UAbs Rel v) )  Rel b)  (open_tm_wrt_tm  v   b ) 
- | Beta_AppAbsIrrel : forall (v:tm),
-     Value  ( (a_UAbs Irrel v) )  ->
-     Beta (a_App  ( (a_UAbs Irrel v) )  Irrel a_Bullet)  (open_tm_wrt_tm  v   a_Bullet ) 
- | Beta_CAppCAbs : forall (a':tm),
-     lc_tm (a_UCAbs a') ->
-     Beta (a_CApp  ( (a_UCAbs a') )  g_Triv)  (open_tm_wrt_co  a'   g_Triv ) 
+     Beta (a_App  ( (a_UAbs psi v) )  psi b)  (open_tm_wrt_tm  v   b ) 
+ | Beta_CAppCAbs : forall (psi:grade) (a':tm),
+     lc_tm (a_UCAbs psi a') ->
+     Beta (a_CApp  ( (a_UCAbs psi a') )  g_Triv)  (open_tm_wrt_co  a'   g_Triv ) 
  | Beta_Axiom : forall (F:tyfam) (a A:tm),
       binds  F  (Ax  a A )   toplevel   ->
      Beta (a_Fam F) a
 with reduction_in_one : tm -> tm -> Prop :=    (* defn reduction_in_one *)
- | E_AbsTerm : forall (L:vars) (a a':tm),
-      ( forall x , x \notin  L  -> reduction_in_one  ( open_tm_wrt_tm a (a_Var_f x) )   ( open_tm_wrt_tm a' (a_Var_f x) )  )  ->
-     reduction_in_one (a_UAbs Irrel a) (a_UAbs Irrel a')
- | E_AppLeft : forall (a b a':tm),
+ | E_AppLeft : forall (a:tm) (psi:grade) (b a':tm),
      lc_tm b ->
      reduction_in_one a a' ->
-     reduction_in_one (a_App a Rel b) (a_App a' Rel b)
- | E_AppLeftIrrel : forall (a a':tm),
-     reduction_in_one a a' ->
-     reduction_in_one (a_App a Irrel a_Bullet) (a_App a' Irrel a_Bullet)
+     reduction_in_one (a_App a psi b) (a_App a' psi b)
  | E_CAppLeft : forall (a a':tm),
      reduction_in_one a a' ->
      reduction_in_one (a_CApp a g_Triv) (a_CApp a' g_Triv)
- | E_AppAbs : forall (v a:tm),
-     lc_tm (a_UAbs Rel v) ->
+ | E_AppAbs : forall (psi:grade) (v a:tm),
+     lc_tm (a_UAbs psi v) ->
      lc_tm a ->
-     reduction_in_one (a_App  ( (a_UAbs Rel v) )  Rel a)  (open_tm_wrt_tm  v   a ) 
- | E_AppAbsIrrel : forall (v:tm),
-     Value  ( (a_UAbs Irrel v) )  ->
-     reduction_in_one (a_App  ( (a_UAbs Irrel v) )  Irrel a_Bullet)  (open_tm_wrt_tm  v   a_Bullet ) 
- | E_CAppCAbs : forall (b:tm),
-     lc_tm (a_UCAbs b) ->
-     reduction_in_one (a_CApp  ( (a_UCAbs b) )  g_Triv)  (open_tm_wrt_co  b   g_Triv ) 
+     reduction_in_one (a_App  ( (a_UAbs psi v) )  psi a)  (open_tm_wrt_tm  v   a ) 
+ | E_CAppCAbs : forall (psi:grade) (b:tm),
+     lc_tm (a_UCAbs psi b) ->
+     reduction_in_one (a_CApp  ( (a_UCAbs psi b) )  g_Triv)  (open_tm_wrt_co  b   g_Triv ) 
  | E_Axiom : forall (F:tyfam) (a A:tm),
       binds  F  (Ax  a A )   toplevel   ->
      reduction_in_one (a_Fam F) a
@@ -1071,192 +1193,204 @@ with reduction : tm -> tm -> Prop :=    (* defn reduction *)
      reduction a a'.
 
 (* defns Jett *)
-Inductive PropWff : context -> constraint -> Prop :=    (* defn PropWff *)
- | E_WffEq : forall (G:context) (a b A:tm),
-     Typing G a A ->
-     Typing G b A ->
-      ( Typing G A a_Star )  ->
-     PropWff G (Eq a b A)
- | E_WffImpl : forall (G:context) (phi1 phi2:constraint),
-     PropWff G phi1 ->
-     PropWff G phi2 ->
-     PropWff G (Impl phi1 phi2)
-with Typing : context -> tm -> tm -> Prop :=    (* defn Typing *)
- | E_Star : forall (G:context),
+Inductive PropWff : context -> grade -> constraint -> Prop :=    (* defn PropWff *)
+ | E_WffEq : forall (G:context) (psi:grade) (a b A:tm),
+     Typing G psi a A ->
+     Typing G psi b A ->
+      ( Typing G psi A a_Star )  ->
+     PropWff G psi (Eq a b A)
+ | E_WffImpl : forall (G:context) (psi:grade) (phi1 phi2:constraint),
+     PropWff G psi phi1 ->
+     PropWff G psi phi2 ->
+     PropWff G psi (Impl phi1 phi2)
+with Typing : context -> grade -> tm -> tm -> Prop :=    (* defn Typing *)
+ | E_Star : forall (G:context) (psi:grade),
      Ctx G ->
-     Typing G a_Star a_Star
- | E_Var : forall (G:context) (x:tmvar) (A:tm),
+     Typing G psi a_Star a_Star
+ | E_Var : forall (G:context) (psi:grade) (x:tmvar) (A:tm) (psi0:grade),
      Ctx G ->
-      binds  x  (Tm  A )  G  ->
-     Typing G (a_Var_f x) A
- | E_Pi : forall (L:vars) (G:context) (rho:relflag) (A B:tm),
-      ( forall x , x \notin  L  -> Typing  (( x ~ Tm  A ) ++  G )   ( open_tm_wrt_tm B (a_Var_f x) )  a_Star )  ->
-      ( Typing G A a_Star )  ->
-     Typing G (a_Pi rho A B) a_Star
- | E_Abs : forall (L:vars) (G:context) (rho:relflag) (a A B:tm),
-      ( forall x , x \notin  L  -> Typing  (( x ~ Tm  A ) ++  G )   ( open_tm_wrt_tm a (a_Var_f x) )   ( open_tm_wrt_tm B (a_Var_f x) )  )  ->
-      ( Typing G A a_Star )  ->
-      ( forall x , x \notin  L  -> RhoCheck rho x  ( open_tm_wrt_tm a (a_Var_f x) )  )  ->
-     Typing G (a_UAbs rho a) (a_Pi rho A B)
- | E_App : forall (G:context) (b a B A:tm),
-     Typing G b (a_Pi Rel A B) ->
-     Typing G a A ->
-     Typing G (a_App b Rel a)  (open_tm_wrt_tm  B   a ) 
- | E_IApp : forall (G:context) (b B a A:tm),
-     Typing G b (a_Pi Irrel A B) ->
-     Typing G a A ->
-     Typing G (a_App b Irrel a_Bullet)  (open_tm_wrt_tm  B   a ) 
- | E_Conv : forall (G:context) (a B A:tm),
-     Typing G a A ->
-     DefEq G  (dom  G )  (Eq A B a_Star) ->
-      ( Typing G B a_Star )  ->
-     Typing G a B
- | E_CPi : forall (L:vars) (G:context) (phi:constraint) (B:tm),
-      ( forall c , c \notin  L  -> Typing  (( c ~ Co  phi ) ++  G )   ( open_tm_wrt_co B (g_Var_f c) )  a_Star )  ->
-      ( PropWff G phi )  ->
-     Typing G (a_CPi phi B) a_Star
- | E_CAbs : forall (L:vars) (G:context) (a:tm) (phi:constraint) (B:tm),
-      ( forall c , c \notin  L  -> Typing  (( c ~ Co  phi ) ++  G )   ( open_tm_wrt_co a (g_Var_f c) )   ( open_tm_wrt_co B (g_Var_f c) )  )  ->
-      ( PropWff G phi )  ->
-     Typing G (a_UCAbs a) (a_CPi phi B)
- | E_CApp : forall (G:context) (a1 B1:tm) (phi:constraint),
-     Typing G a1 (a_CPi phi B1) ->
-     DefEq G  (dom  G )  phi ->
-     Typing G (a_CApp a1 g_Triv)  (open_tm_wrt_co  B1   g_Triv ) 
- | E_Fam : forall (G:context) (F:tyfam) (A a:tm),
+      ( psi0  <=  psi )  ->
+      binds  x  ( psi0 , (Tm  A ))  G  ->
+     Typing G psi (a_Var_f x) A
+ | E_Pi : forall (L:vars) (G:context) (psi psi0:grade) (A B:tm),
+      ( forall x , x \notin  L  -> Typing  (( x ~ ( psi , Tm  A )) ++  G )  psi  ( open_tm_wrt_tm B (a_Var_f x) )  a_Star )  ->
+      ( Typing G psi A a_Star )  ->
+     Typing G psi (a_Pi psi0 A B) a_Star
+ | E_Abs : forall (L:vars) (G:context) (psi psi0:grade) (a A B:tm),
+      ( forall x , x \notin  L  -> Typing  (( x ~ (  (q_join  psi0   psi )  , Tm  A )) ++  G )  psi  ( open_tm_wrt_tm a (a_Var_f x) )   ( open_tm_wrt_tm B (a_Var_f x) )  )  ->
+      ( Typing  (meet_ctx_l   q_C    G )   q_C  A a_Star )  ->
+     Typing G psi (a_UAbs psi0 a) (a_Pi psi0 A B)
+ | E_App : forall (G:context) (psi:grade) (b:tm) (psi0:grade) (a B A:tm),
+     Typing G psi b (a_Pi psi0 A B) ->
+     Typing G  (q_join  psi0   psi )  a A ->
+      ( psi0  <=   q_C  )  ->
+     Typing G psi (a_App b psi0 a)  (open_tm_wrt_tm  B   a ) 
+ | E_AppIrrel : forall (G:context) (psi:grade) (b:tm) (psi0:grade) (a B A:tm),
+     Typing G psi b (a_Pi psi0 A B) ->
+     Typing  (meet_ctx_l   q_C    G )   q_C  a A ->
+      (  q_C   <  psi0 )  ->
+     Typing G psi (a_App b psi0 a)  (open_tm_wrt_tm  B   a ) 
+ | E_Conv : forall (G:context) (psi:grade) (a B A:tm),
+     Typing G psi a A ->
+     DefEq  (meet_ctx_l   q_C    G )   q_C  (Eq A B a_Star) ->
+      ( Typing  (meet_ctx_l   q_C    G )   q_C  B a_Star )  ->
+     Typing G psi a B
+ | E_CPi : forall (L:vars) (G:context) (psi psi0:grade) (phi:constraint) (B:tm),
+      ( forall c , c \notin  L  -> Typing  (( c ~ ( psi , Co  phi )) ++  G )  psi  ( open_tm_wrt_co B (g_Var_f c) )  a_Star )  ->
+      ( PropWff G psi phi )  ->
+     Typing G psi (a_CPi psi0 phi B) a_Star
+ | E_CAbs : forall (L:vars) (G:context) (psi psi0:grade) (a:tm) (phi:constraint) (B:tm),
+      ( forall c , c \notin  L  -> Typing  (( c ~ (  (q_join  psi0   psi )  , Co  phi )) ++  G )  psi  ( open_tm_wrt_co a (g_Var_f c) )   ( open_tm_wrt_co B (g_Var_f c) )  )  ->
+      ( PropWff  (meet_ctx_l   q_C    G )   q_C  phi )  ->
+     Typing G psi (a_UCAbs psi0 a) (a_CPi psi0 phi B)
+ | E_CApp : forall (G:context) (psi:grade) (a1 B1:tm) (phi:constraint),
+     Typing G psi a1 (a_CPi  q_Top  phi B1) ->
+     DefEq  (meet_ctx_l   q_C    G )   q_C  phi ->
+     Typing G psi (a_CApp a1 g_Triv)  (open_tm_wrt_co  B1   g_Triv ) 
+ | E_Fam : forall (G:context) (psi:grade) (F:tyfam) (A a:tm),
+      (  q_C   <=  psi )  ->
      Ctx G ->
       binds  F  (Ax  a A )   toplevel   ->
-      ( Typing  nil  A a_Star )  ->
-     Typing G (a_Fam F) A
-with Iso : context -> available_props -> constraint -> constraint -> Prop :=    (* defn Iso *)
- | E_PropCong : forall (G:context) (D:available_props) (A1 B1 A A2 B2:tm),
-     DefEq G D (Eq A1 A2 A) ->
-     DefEq G D (Eq B1 B2 A) ->
-     Iso G D (Eq A1 B1 A) (Eq A2 B2 A)
- | E_IsoConv : forall (G:context) (D:available_props) (A1 A2 A B:tm),
-     DefEq G D (Eq A B a_Star) ->
-     PropWff G (Eq A1 A2 A) ->
-     PropWff G (Eq A1 A2 B) ->
-     Iso G D (Eq A1 A2 A) (Eq A1 A2 B)
- | E_CPiFst : forall (G:context) (D:available_props) (phi1 phi2:constraint) (B1 B2:tm),
-     DefEq G D (Eq (a_CPi phi1 B1) (a_CPi phi2 B2) a_Star) ->
-     Iso G D phi1 phi2
- | E_ImplCong : forall (G:context) (D:available_props) (phi1 phi3 phi2 phi4:constraint),
-     Iso G D phi1 phi2 ->
-     Iso G D phi3 phi4 ->
-     Iso G D (Impl phi1 phi3) (Impl phi2 phi4)
-with DefEq : context -> available_props -> constraint -> Prop :=    (* defn DefEq *)
- | E_Assn : forall (G:context) (D:available_props) (phi:constraint) (c:covar),
+      ( Typing  nil   q_C  A a_Star )  ->
+     Typing G psi (a_Fam F) A
+with Iso : context -> grade -> constraint -> constraint -> Prop :=    (* defn Iso *)
+ | E_PropCong : forall (G:context) (psi:grade) (A1 B1 A A2 B2:tm),
+     DefEq G psi (Eq A1 A2 A) ->
+     DefEq G psi (Eq B1 B2 A) ->
+     Iso G psi (Eq A1 B1 A) (Eq A2 B2 A)
+ | E_IsoConv : forall (G:context) (psi:grade) (A1 A2 A B:tm),
+     DefEq G psi (Eq A B a_Star) ->
+     PropWff G psi (Eq A1 A2 A) ->
+     PropWff G psi (Eq A1 A2 B) ->
+     Iso G psi (Eq A1 A2 A) (Eq A1 A2 B)
+ | E_CPiFst : forall (G:context) (psi:grade) (phi1 phi2:constraint) (psi0:grade) (B1 B2:tm),
+     DefEq G psi (Eq (a_CPi psi0 phi1 B1) (a_CPi psi0 phi2 B2) a_Star) ->
+     Iso G psi phi1 phi2
+ | E_ImplCong : forall (G:context) (psi:grade) (phi1 phi3 phi2 phi4:constraint),
+     Iso G psi phi1 phi2 ->
+     Iso G psi phi3 phi4 ->
+     Iso G psi (Impl phi1 phi3) (Impl phi2 phi4)
+with CDefEq : context -> grade -> grade -> tm -> tm -> tm -> Prop :=    (* defn CDefEq *)
+ | CDefEq_Leq : forall (G:context) (psi psi0:grade) (a b A:tm),
+      ( psi0  <=  psi )  ->
+     DefEq G psi (Eq a b A) ->
+     CDefEq G psi psi0 a b A
+ | CDefEq_Nleq : forall (G:context) (psi psi0:grade) (a b A:tm),
+      not (  (  ( psi0  <=  psi )  )  )  ->
      Ctx G ->
-      binds  c  (Co  phi )  G  ->
-      AtomSetImpl.In  c   D  ->
-     DefEq G D phi
- | E_Refl : forall (G:context) (D:available_props) (a A:tm),
-     Typing G a A ->
-     DefEq G D (Eq a a A)
- | E_Sym : forall (G:context) (D:available_props) (a b A:tm),
-     DefEq G D (Eq b a A) ->
-     DefEq G D (Eq a b A)
- | E_Trans : forall (G:context) (D:available_props) (a b A a1:tm),
-     DefEq G D (Eq a a1 A) ->
-     DefEq G D (Eq a1 b A) ->
-     DefEq G D (Eq a b A)
- | E_Beta : forall (G:context) (D:available_props) (a1 a2 B:tm),
-     Typing G a1 B ->
-      ( Typing G a2 B )  ->
+      ( psi0  <=   q_C  )  ->
+     Typing G  (q_join  psi0   psi )  a A ->
+     Typing G  (q_join  psi0   psi )  b A ->
+     CDefEq G psi psi0 a b A
+ | CDefEq_NleqIrrel : forall (G:context) (psi psi0:grade) (a b A:tm),
+      not (  (  ( psi0  <=  psi )  )  )  ->
+     Ctx G ->
+      (  q_C   <  psi0 )  ->
+     Typing  (meet_ctx_l   q_C    G )   q_C  a A ->
+     Typing  (meet_ctx_l   q_C    G )   q_C  b A ->
+     CDefEq G psi psi0 a b A
+with DefEq : context -> grade -> constraint -> Prop :=    (* defn DefEq *)
+ | E_Assn : forall (G:context) (psi:grade) (phi:constraint) (psi0:grade) (c:covar),
+     Ctx G ->
+      ( psi0  <=  psi )  ->
+      binds  c  ( psi0 , (Co  phi ))  G  ->
+     DefEq G psi phi
+ | E_Refl : forall (G:context) (psi:grade) (a A:tm),
+     Typing G psi a A ->
+     DefEq G psi (Eq a a A)
+ | E_Sym : forall (G:context) (psi:grade) (a b A:tm),
+     DefEq G psi (Eq b a A) ->
+     DefEq G psi (Eq a b A)
+ | E_Trans : forall (G:context) (psi:grade) (a b A a1:tm),
+     DefEq G psi (Eq a a1 A) ->
+     DefEq G psi (Eq a1 b A) ->
+     DefEq G psi (Eq a b A)
+ | E_Beta : forall (G:context) (psi:grade) (a1 a2 B:tm),
+     Typing G psi a1 B ->
+      ( Typing G psi a2 B )  ->
      Beta a1 a2 ->
-     DefEq G D (Eq a1 a2 B)
- | E_PiCong : forall (L:vars) (G:context) (D:available_props) (rho:relflag) (A1 B1 A2 B2:tm),
-     DefEq G D (Eq A1 A2 a_Star) ->
-      ( forall x , x \notin  L  -> DefEq  (( x ~ Tm  A1 ) ++  G )  D (Eq  ( open_tm_wrt_tm B1 (a_Var_f x) )   ( open_tm_wrt_tm B2 (a_Var_f x) )  a_Star) )  ->
-      ( Typing G A1 a_Star )  ->
-      ( Typing G (a_Pi rho A1 B1) a_Star )  ->
-      ( Typing G (a_Pi rho A2 B2) a_Star )  ->
-     DefEq G D (Eq  ( (a_Pi rho A1 B1) )   ( (a_Pi rho A2 B2) )  a_Star)
- | E_AbsCong : forall (L:vars) (G:context) (D:available_props) (rho:relflag) (b1 b2 A1 B:tm),
-      ( forall x , x \notin  L  -> DefEq  (( x ~ Tm  A1 ) ++  G )  D (Eq  ( open_tm_wrt_tm b1 (a_Var_f x) )   ( open_tm_wrt_tm b2 (a_Var_f x) )   ( open_tm_wrt_tm B (a_Var_f x) ) ) )  ->
-      ( Typing G A1 a_Star )  ->
-      ( forall x , x \notin  L  -> RhoCheck rho x  ( open_tm_wrt_tm b1 (a_Var_f x) )  )  ->
-      ( forall x , x \notin  L  -> RhoCheck rho x  ( open_tm_wrt_tm b2 (a_Var_f x) )  )  ->
-     DefEq G D (Eq  ( (a_UAbs rho b1) )   ( (a_UAbs rho b2) )  (a_Pi rho A1 B))
- | E_AppCong : forall (G:context) (D:available_props) (a1 a2 b1 b2 B A:tm),
-     DefEq G D (Eq a1 b1 (a_Pi Rel A B)) ->
-     DefEq G D (Eq a2 b2 A) ->
-     DefEq G D (Eq (a_App a1 Rel a2) (a_App b1 Rel b2)  (  (open_tm_wrt_tm  B   a2 )  ) )
- | E_IAppCong : forall (G:context) (D:available_props) (a1 b1 B a A:tm),
-     DefEq G D (Eq a1 b1 (a_Pi Irrel A B)) ->
-     Typing G a A ->
-     DefEq G D (Eq (a_App a1 Irrel a_Bullet) (a_App b1 Irrel a_Bullet)  (  (open_tm_wrt_tm  B   a )  ) )
- | E_PiFst : forall (G:context) (D:available_props) (A1 A2:tm) (rho:relflag) (B1 B2:tm),
-     DefEq G D (Eq (a_Pi rho A1 B1) (a_Pi rho A2 B2) a_Star) ->
-     DefEq G D (Eq A1 A2 a_Star)
- | E_PiSnd : forall (G:context) (D:available_props) (B1 a1 B2 a2:tm) (rho:relflag) (A1 A2:tm),
-     DefEq G D (Eq (a_Pi rho A1 B1) (a_Pi rho A2 B2) a_Star) ->
-     DefEq G D (Eq a1 a2 A1) ->
-     DefEq G D (Eq  (open_tm_wrt_tm  B1   a1 )   (open_tm_wrt_tm  B2   a2 )  a_Star)
- | E_CPiCong : forall (L:vars) (G:context) (D:available_props) (phi1:constraint) (A:tm) (phi2:constraint) (B:tm),
-     Iso G D phi1 phi2 ->
-      ( forall c , c \notin  L  -> DefEq  (( c ~ Co  phi1 ) ++  G )  D (Eq  ( open_tm_wrt_co A (g_Var_f c) )   ( open_tm_wrt_co B (g_Var_f c) )  a_Star) )  ->
-      ( PropWff G phi1 )  ->
-      ( Typing G (a_CPi phi1 A) a_Star )  ->
-      ( Typing G (a_CPi phi2 B) a_Star )  ->
-     DefEq G D (Eq (a_CPi phi1 A) (a_CPi phi2 B) a_Star)
- | E_CAbsCong : forall (L:vars) (G:context) (D:available_props) (a b:tm) (phi1:constraint) (B:tm),
-      ( forall c , c \notin  L  -> DefEq  (( c ~ Co  phi1 ) ++  G )  D (Eq  ( open_tm_wrt_co a (g_Var_f c) )   ( open_tm_wrt_co b (g_Var_f c) )   ( open_tm_wrt_co B (g_Var_f c) ) ) )  ->
-      ( PropWff G phi1 )  ->
-     DefEq G D (Eq  ( (a_UCAbs a) )   ( (a_UCAbs b) )  (a_CPi phi1 B))
- | E_CAppCong : forall (G:context) (D:available_props) (a1 b1 B:tm) (phi:constraint),
-     DefEq G D (Eq a1 b1 (a_CPi phi B)) ->
-     DefEq G  (dom  G )  phi ->
-     DefEq G D (Eq (a_CApp a1 g_Triv) (a_CApp b1 g_Triv)  (open_tm_wrt_co  B   g_Triv ) )
- | E_CPiSnd : forall (G:context) (D:available_props) (B1 B2:tm) (phi1 phi2:constraint),
-     DefEq G D (Eq (a_CPi phi1 B1) (a_CPi phi2 B2) a_Star) ->
-     DefEq G  (dom  G )  phi1 ->
-     DefEq G  (dom  G )  phi2 ->
-     DefEq G D (Eq  (open_tm_wrt_co  B1   g_Triv )   (open_tm_wrt_co  B2   g_Triv )  a_Star)
- | E_Cast : forall (G:context) (D:available_props) (phi2 phi1:constraint),
-     DefEq G D phi1 ->
-     Iso G D phi1 phi2 ->
-     DefEq G D phi2
- | E_EqConv : forall (G:context) (D:available_props) (a b B A:tm),
-     DefEq G D (Eq a b A) ->
-     DefEq G  (dom  G )  (Eq A B a_Star) ->
-     DefEq G D (Eq a b B)
- | E_IsoSnd : forall (G:context) (D:available_props) (A A' a b a' b':tm),
-     Iso G D (Eq a b A) (Eq a' b' A') ->
-     DefEq G D (Eq A A' a_Star)
- | E_EtaRel : forall (L:vars) (G:context) (D:available_props) (a b A B:tm),
-     Typing G b (a_Pi Rel A B) ->
-      ( forall x , x \notin  L  ->  (  ( open_tm_wrt_tm a (a_Var_f x) )   =  (a_App b Rel (a_Var_f x)) )  )  ->
-     DefEq G D (Eq (a_UAbs Rel a) b (a_Pi Rel A B))
- | E_EtaIrrel : forall (L:vars) (G:context) (D:available_props) (a b A B:tm),
-     Typing G b (a_Pi Irrel A B) ->
-      ( forall x , x \notin  L  ->  (  ( open_tm_wrt_tm a (a_Var_f x) )   =  (a_App b Irrel a_Bullet) )  )  ->
-     DefEq G D (Eq (a_UAbs Irrel a) b (a_Pi Irrel A B))
- | E_EtaC : forall (L:vars) (G:context) (D:available_props) (a b:tm) (phi:constraint) (B:tm),
-     Typing G b (a_CPi phi B) ->
+     DefEq G psi (Eq a1 a2 B)
+ | E_PiCong : forall (L:vars) (G:context) (psi psi0:grade) (A1 B1 A2 B2:tm),
+     DefEq G psi (Eq A1 A2 a_Star) ->
+      ( forall x , x \notin  L  -> DefEq  (( x ~ ( psi , Tm  A1 )) ++  G )  psi (Eq  ( open_tm_wrt_tm B1 (a_Var_f x) )   ( open_tm_wrt_tm B2 (a_Var_f x) )  a_Star) )  ->
+      ( Typing G psi A1 a_Star )  ->
+      ( Typing G psi (a_Pi psi0 A1 B1) a_Star )  ->
+      ( Typing G psi (a_Pi psi0 A2 B2) a_Star )  ->
+     DefEq G psi (Eq  ( (a_Pi psi0 A1 B1) )   ( (a_Pi psi0 A2 B2) )  a_Star)
+ | E_AbsCong : forall (L:vars) (G:context) (psi psi0:grade) (b1 b2 A1 B:tm),
+      ( forall x , x \notin  L  -> DefEq  (( x ~ (  (q_join  psi0   psi )  , Tm  A1 )) ++  G )  psi (Eq  ( open_tm_wrt_tm b1 (a_Var_f x) )   ( open_tm_wrt_tm b2 (a_Var_f x) )   ( open_tm_wrt_tm B (a_Var_f x) ) ) )  ->
+      ( Typing  (meet_ctx_l   q_C    G )   q_C  A1 a_Star )  ->
+     DefEq G psi (Eq  ( (a_UAbs psi0 b1) )   ( (a_UAbs psi0 b2) )  (a_Pi psi0 A1 B))
+ | E_AppCong : forall (G:context) (psi:grade) (a1:tm) (psi0:grade) (a2 b1 b2 B A:tm),
+     DefEq G psi (Eq a1 b1 (a_Pi psi0 A B)) ->
+     CDefEq G psi psi0 a2 b2 A ->
+     DefEq G psi (Eq (a_App a1 psi0 a2) (a_App b1 psi0 b2)  (  (open_tm_wrt_tm  B   a2 )  ) )
+ | E_PiFst : forall (G:context) (psi:grade) (A1 A2:tm) (psi0:grade) (B1 B2:tm),
+     DefEq G psi (Eq (a_Pi psi0 A1 B1) (a_Pi psi0 A2 B2) a_Star) ->
+     DefEq G psi (Eq A1 A2 a_Star)
+ | E_PiSnd : forall (G:context) (psi:grade) (B1 a1 B2 a2:tm) (psi0:grade) (A1 A2:tm),
+     DefEq G psi (Eq (a_Pi psi0 A1 B1) (a_Pi psi0 A2 B2) a_Star) ->
+     DefEq G psi (Eq a1 a2 A1) ->
+     DefEq G psi (Eq  (open_tm_wrt_tm  B1   a1 )   (open_tm_wrt_tm  B2   a2 )  a_Star)
+ | E_CPiCong : forall (L:vars) (G:context) (psi psi0:grade) (phi1:constraint) (A:tm) (phi2:constraint) (B:tm),
+     Iso G psi phi1 phi2 ->
+      ( forall c , c \notin  L  -> DefEq  (( c ~ ( psi , Co  phi1 )) ++  G )  psi (Eq  ( open_tm_wrt_co A (g_Var_f c) )   ( open_tm_wrt_co B (g_Var_f c) )  a_Star) )  ->
+      ( PropWff G psi phi1 )  ->
+      ( Typing G psi (a_CPi psi0 phi1 A) a_Star )  ->
+      ( Typing G psi (a_CPi psi0 phi2 B) a_Star )  ->
+     DefEq G psi (Eq (a_CPi psi0 phi1 A) (a_CPi psi0 phi2 B) a_Star)
+ | E_CAbsCong : forall (L:vars) (G:context) (psi psi0:grade) (a b:tm) (phi1:constraint) (B:tm),
+      ( forall c , c \notin  L  -> DefEq  (( c ~ (  (q_join  psi0   psi )  , Co  phi1 )) ++  G )  psi (Eq  ( open_tm_wrt_co a (g_Var_f c) )   ( open_tm_wrt_co b (g_Var_f c) )   ( open_tm_wrt_co B (g_Var_f c) ) ) )  ->
+      ( PropWff  (meet_ctx_l   q_C    G )   q_C  phi1 )  ->
+     DefEq G psi (Eq  ( (a_UCAbs psi0 a) )   ( (a_UCAbs psi0 b) )  (a_CPi psi0 phi1 B))
+ | E_CAppCong : forall (G:context) (psi:grade) (a1 b1 B:tm) (phi:constraint),
+     DefEq G psi (Eq a1 b1 (a_CPi  q_Top  phi B)) ->
+     DefEq  (meet_ctx_l   q_C    G )   q_C  phi ->
+     DefEq G psi (Eq (a_CApp a1 g_Triv) (a_CApp b1 g_Triv)  (open_tm_wrt_co  B   g_Triv ) )
+ | E_CPiSnd : forall (G:context) (psi:grade) (B1 B2:tm) (psi0:grade) (phi1 phi2:constraint),
+     DefEq G psi (Eq (a_CPi psi0 phi1 B1) (a_CPi psi0 phi2 B2) a_Star) ->
+     DefEq  (meet_ctx_l   q_C    G )   q_C  phi1 ->
+     DefEq  (meet_ctx_l   q_C    G )   q_C  phi2 ->
+     DefEq G psi (Eq  (open_tm_wrt_co  B1   g_Triv )   (open_tm_wrt_co  B2   g_Triv )  a_Star)
+ | E_Cast : forall (G:context) (psi:grade) (phi2 phi1:constraint),
+     DefEq G psi phi1 ->
+     Iso G psi phi1 phi2 ->
+     DefEq G psi phi2
+ | E_EqConv : forall (G:context) (psi:grade) (a b B A:tm),
+     DefEq G psi (Eq a b A) ->
+     DefEq  (meet_ctx_l   q_C    G )  psi (Eq A B a_Star) ->
+     DefEq G psi (Eq a b B)
+ | E_IsoSnd : forall (G:context) (psi:grade) (A A' a b a' b':tm),
+     Iso G psi (Eq a b A) (Eq a' b' A') ->
+     DefEq G psi (Eq A A' a_Star)
+ | E_EtaRel : forall (L:vars) (G:context) (psi psi0:grade) (a b A B:tm),
+     Typing G psi b (a_Pi psi0 A B) ->
+      ( forall x , x \notin  L  ->  (  ( open_tm_wrt_tm a (a_Var_f x) )   =  (a_App b psi0 (a_Var_f x)) )  )  ->
+     DefEq G psi (Eq (a_UAbs psi0 a) b (a_Pi psi0 A B))
+ | E_EtaC : forall (L:vars) (G:context) (psi:grade) (a b:tm) (phi:constraint) (B:tm),
+     Typing G psi b (a_CPi  q_Top  phi B) ->
       ( forall c , c \notin  L  ->  (  ( open_tm_wrt_co a (g_Var_f c) )   =  (a_CApp b g_Triv) )  )  ->
-     DefEq G D (Eq (a_UCAbs a) b (a_CPi phi B))
- | E_ImplApp : forall (G:context) (D:available_props) (phi2 phi1:constraint),
-     DefEq G D (Impl phi1 phi2) ->
-     DefEq G D phi1 ->
-     DefEq G D phi2
- | E_ImplAbs : forall (G:context) (D:available_props) (phi1 phi2:constraint) (c:covar),
-     DefEq  (( c ~ Co  phi1 ) ++  G )   (singleton  c  \u  D )  phi2 ->
-     DefEq G D (Impl phi1 phi2)
+     DefEq G psi (Eq (a_UCAbs  q_Top  a) b (a_CPi  q_Top  phi B))
+ | E_ImplApp : forall (G:context) (psi:grade) (phi2 phi1:constraint),
+     DefEq G psi (Impl phi1 phi2) ->
+     DefEq G psi phi1 ->
+     DefEq G psi phi2
+ | E_ImplAbs : forall (G:context) (psi:grade) (phi1 phi2:constraint) (c:covar),
+     DefEq  (( c ~ (  q_C  , Co  phi1 )) ++  G )  psi phi2 ->
+     DefEq G psi (Impl phi1 phi2)
 with Ctx : context -> Prop :=    (* defn Ctx *)
  | E_Empty : 
      Ctx  nil 
- | E_ConsTm : forall (G:context) (x:tmvar) (A:tm),
+ | E_ConsTm : forall (G:context) (x:tmvar) (psi:grade) (A:tm),
      Ctx G ->
-     Typing G A a_Star ->
+     Typing  (meet_ctx_l   q_C    G )   q_C  A a_Star ->
       ~ AtomSetImpl.In  x  (dom  G )  ->
-     Ctx  (( x ~ Tm  A ) ++  G ) 
- | E_ConsCo : forall (G:context) (c:covar) (phi:constraint),
+     Ctx  (( x ~ ( psi , Tm  A )) ++  G ) 
+ | E_ConsCo : forall (G:context) (c:covar) (psi:grade) (phi:constraint),
      Ctx G ->
-     PropWff G phi ->
+     PropWff  (meet_ctx_l   q_C    G )   q_C  phi ->
       ~ AtomSetImpl.In  c  (dom  G )  ->
-     Ctx  (( c ~ Co  phi ) ++  G ) .
+     Ctx  (( c ~ ( psi , Co  phi )) ++  G ) .
 
 (* defns Jsig *)
 Inductive Sig : sig -> Prop :=    (* defn Sig *)
@@ -1264,240 +1398,242 @@ Inductive Sig : sig -> Prop :=    (* defn Sig *)
      Sig  nil 
  | Sig_ConsAx : forall (S:sig) (F:tyfam) (a A:tm),
      Sig S ->
-     Typing  nil  A a_Star ->
-     Typing  nil  a A ->
+     Typing  nil   q_C  A a_Star ->
+     Typing  nil   q_C  a A ->
       ~ AtomSetImpl.In  F  (dom  S )  ->
      Sig  (( F ~ Ax a A )++ S ) .
 
 (* defns Jann *)
-Inductive AnnPropWff : context -> constraint -> Prop :=    (* defn AnnPropWff *)
- | An_Wff : forall (G:context) (a b A B:tm),
-     AnnTyping G a A ->
-     AnnTyping G b B ->
+Inductive AnnPropWff : context -> grade -> constraint -> Prop :=    (* defn AnnPropWff *)
+ | An_Wff : forall (G:context) (psi:grade) (a b A B:tm),
+     AnnTyping G psi a A ->
+     AnnTyping G psi b B ->
       (  (erase_tm  A )   =   (erase_tm  B )  )  ->
-     AnnPropWff G (Eq a b A)
-with AnnTyping : context -> tm -> tm -> Prop :=    (* defn AnnTyping *)
- | An_Star : forall (G:context),
+     AnnPropWff G psi (Eq a b A)
+with AnnTyping : context -> grade -> tm -> tm -> Prop :=    (* defn AnnTyping *)
+ | An_Star : forall (G:context) (psi:grade),
      AnnCtx G ->
-     AnnTyping G a_Star a_Star
- | An_Var : forall (G:context) (x:tmvar) (A:tm),
+     AnnTyping G psi a_Star a_Star
+ | An_Var : forall (G:context) (psi:grade) (x:tmvar) (A:tm) (psi0:grade),
      AnnCtx G ->
-      binds  x  (Tm  A )  G  ->
-     AnnTyping G (a_Var_f x) A
- | An_Pi : forall (L:vars) (G:context) (rho:relflag) (A B:tm),
-      ( forall x , x \notin  L  -> AnnTyping  (( x ~ Tm  A ) ++  G )   ( open_tm_wrt_tm B (a_Var_f x) )  a_Star )  ->
-      ( AnnTyping G A a_Star )  ->
-     AnnTyping G (a_Pi rho A B) a_Star
- | An_Abs : forall (L:vars) (G:context) (rho:relflag) (A a B:tm),
-      ( AnnTyping G A a_Star )  ->
-      ( forall x , x \notin  L  -> AnnTyping  (( x ~ Tm  A ) ++  G )   ( open_tm_wrt_tm a (a_Var_f x) )   ( open_tm_wrt_tm B (a_Var_f x) )  )  ->
-      ( forall x , x \notin  L  -> RhoCheck rho x  (erase_tm   ( open_tm_wrt_tm a (a_Var_f x) )  )  )  ->
-     AnnTyping G (a_Abs rho A a) (a_Pi rho A B)
- | An_App : forall (G:context) (b:tm) (rho:relflag) (a B A:tm),
-     AnnTyping G b (a_Pi rho A B) ->
-     AnnTyping G a A ->
-     AnnTyping G (a_App b rho a)  (open_tm_wrt_tm  B   a ) 
- | An_Conv : forall (G:context) (a:tm) (g:co) (B A:tm),
-     AnnTyping G a A ->
-     AnnDefEq G  (dom  G )  g A B ->
-     AnnTyping G B a_Star ->
-     AnnTyping G (a_Conv a g) B
- | An_CPi : forall (L:vars) (G:context) (phi:constraint) (B:tm),
-      ( AnnPropWff G phi )  ->
-      ( forall c , c \notin  L  -> AnnTyping  (( c ~ Co  phi ) ++  G )   ( open_tm_wrt_co B (g_Var_f c) )  a_Star )  ->
-     AnnTyping G (a_CPi phi B) a_Star
- | An_CAbs : forall (L:vars) (G:context) (phi:constraint) (a B:tm),
-      ( AnnPropWff G phi )  ->
-      ( forall c , c \notin  L  -> AnnTyping  (( c ~ Co  phi ) ++  G )   ( open_tm_wrt_co a (g_Var_f c) )   ( open_tm_wrt_co B (g_Var_f c) )  )  ->
-     AnnTyping G (a_CAbs phi a) (a_CPi phi B)
- | An_CApp : forall (G:context) (a1:tm) (g:co) (B a b A1:tm),
-     AnnTyping G a1 (a_CPi (Eq a b A1) B) ->
-     AnnDefEq G  (dom  G )  g a b ->
-     AnnTyping G (a_CApp a1 g)  (open_tm_wrt_co  B   g ) 
- | An_Fam : forall (G:context) (F:tyfam) (A a:tm),
+      binds  x  ( psi0 , (Tm  A ))  G  ->
+      ( psi0  <=  psi )  ->
+     AnnTyping G psi (a_Var_f x) A
+ | An_Pi : forall (L:vars) (G:context) (psi psi0:grade) (A B:tm),
+      ( forall x , x \notin  L  -> AnnTyping  (( x ~ ( psi , Tm  A )) ++  G )  psi  ( open_tm_wrt_tm B (a_Var_f x) )  a_Star )  ->
+      ( AnnTyping G psi A a_Star )  ->
+     AnnTyping G psi (a_Pi psi0 A B) a_Star
+ | An_Abs : forall (L:vars) (G:context) (psi psi0:grade) (A a B:tm),
+      ( AnnTyping  (meet_ctx_l   q_C    G )   q_C  A a_Star )  ->
+      ( forall x , x \notin  L  -> AnnTyping  (( x ~ (  (q_join  psi0   psi )  , Tm  A )) ++  G )  psi  ( open_tm_wrt_tm a (a_Var_f x) )   ( open_tm_wrt_tm B (a_Var_f x) )  )  ->
+     AnnTyping G psi (a_Abs psi0 A a) (a_Pi psi0 A B)
+ | An_App : forall (G:context) (psi:grade) (b:tm) (psi0:grade) (a B A:tm),
+     AnnTyping G psi b (a_Pi psi0 A B) ->
+     AnnTyping G  (q_join  psi0   psi )  a A ->
+      ( psi0  <=   q_C  )  ->
+     AnnTyping G psi (a_App b psi0 a)  (open_tm_wrt_tm  B   a ) 
+ | An_AppIrrel : forall (G:context) (psi:grade) (b:tm) (psi0:grade) (a B A:tm),
+     AnnTyping G psi b (a_Pi psi0 A B) ->
+     AnnTyping  (meet_ctx_l   q_C    G )   q_C  a A ->
+      (  q_C   <  psi0 )  ->
+     AnnTyping G psi (a_App b psi0 a)  (open_tm_wrt_tm  B   a ) 
+ | An_Conv : forall (G:context) (psi:grade) (a:tm) (g:co) (B A:tm),
+     AnnTyping G psi a A ->
+     AnnDefEq  (meet_ctx_l   q_C    G )   q_C  g A B ->
+     AnnTyping  (meet_ctx_l   q_C    G )   q_C  B a_Star ->
+     AnnTyping G psi (a_Conv a g) B
+ | An_CPi : forall (L:vars) (G:context) (psi psi0:grade) (phi:constraint) (B:tm),
+      ( AnnPropWff G psi phi )  ->
+      ( forall c , c \notin  L  -> AnnTyping  (( c ~ ( psi , Co  phi )) ++  G )  psi  ( open_tm_wrt_co B (g_Var_f c) )  a_Star )  ->
+     AnnTyping G psi (a_CPi psi0 phi B) a_Star
+ | An_CAbs : forall (L:vars) (G:context) (psi psi0:grade) (phi:constraint) (a B:tm),
+      ( AnnPropWff  (meet_ctx_l   q_C    G )   q_C  phi )  ->
+      ( forall c , c \notin  L  -> AnnTyping  (( c ~ (  (q_join  psi0   psi )  , Co  phi )) ++  G )  psi  ( open_tm_wrt_co a (g_Var_f c) )   ( open_tm_wrt_co B (g_Var_f c) )  )  ->
+     AnnTyping G psi (a_CAbs psi0 phi a) (a_CPi psi0 phi B)
+ | An_CApp : forall (G:context) (psi:grade) (a1:tm) (g:co) (B a b A1:tm),
+     AnnTyping G psi a1 (a_CPi  q_Top  (Eq a b A1) B) ->
+     AnnDefEq  (meet_ctx_l   q_C    G )   q_C  g a b ->
+     AnnTyping G psi (a_CApp a1 g)  (open_tm_wrt_co  B   g ) 
+ | An_Fam : forall (G:context) (psi:grade) (F:tyfam) (A a:tm),
      AnnCtx G ->
+      (  q_C   <=  psi )  ->
       binds  F  (Ax  a A )   an_toplevel   ->
-      ( AnnTyping  nil  A a_Star )  ->
-     AnnTyping G (a_Fam F) A
-with AnnIso : context -> available_props -> co -> constraint -> constraint -> Prop :=    (* defn AnnIso *)
- | An_PropCong : forall (G:context) (D:available_props) (g1:co) (A:tm) (g2:co) (A1 B1 A2 B2:tm),
-     AnnDefEq G D g1 A1 A2 ->
-     AnnDefEq G D g2 B1 B2 ->
-     AnnPropWff G (Eq A1 B1 A) ->
-     AnnPropWff G (Eq A2 B2 A) ->
-     AnnIso G D  ( (g_EqCong g1 A g2) )   ( (Eq A1 B1 A) )   ( (Eq A2 B2 A) ) 
- | An_CPiFst : forall (G:context) (D:available_props) (g:co) (phi1 phi2:constraint) (A2 B2:tm),
-     AnnDefEq G D g (a_CPi phi1 A2) (a_CPi phi2 B2) ->
-     AnnIso G D (g_CPiFst g) phi1 phi2
- | An_IsoSym : forall (G:context) (D:available_props) (g:co) (phi2 phi1:constraint),
-     AnnIso G D g phi1 phi2 ->
-     AnnIso G D (g_Sym g) phi2 phi1
- | An_IsoConv : forall (G:context) (D:available_props) (a1 a2 A a1' a2' B:tm) (g:co),
-     AnnDefEq G D g A B ->
-     AnnPropWff G (Eq a1 a2 A) ->
-     AnnPropWff G (Eq a1' a2' B) ->
+      ( AnnTyping  nil   q_C  A a_Star )  ->
+     AnnTyping G psi (a_Fam F) A
+with AnnIso : context -> grade -> co -> constraint -> constraint -> Prop :=    (* defn AnnIso *)
+ | An_PropCong : forall (G:context) (psi:grade) (g1:co) (A:tm) (g2:co) (A1 B1 A2 B2:tm),
+     AnnDefEq G psi g1 A1 A2 ->
+     AnnDefEq G psi g2 B1 B2 ->
+     AnnPropWff G psi (Eq A1 B1 A) ->
+     AnnPropWff G psi (Eq A2 B2 A) ->
+     AnnIso G psi  ( (g_EqCong g1 A g2) )   ( (Eq A1 B1 A) )   ( (Eq A2 B2 A) ) 
+ | An_CPiFst : forall (G:context) (psi:grade) (g:co) (phi1 phi2:constraint) (psi0:grade) (A2 B2:tm),
+     AnnDefEq G psi g (a_CPi psi0 phi1 A2) (a_CPi psi0 phi2 B2) ->
+     AnnIso G psi (g_CPiFst g) phi1 phi2
+ | An_IsoSym : forall (G:context) (psi:grade) (g:co) (phi2 phi1:constraint),
+     AnnIso G psi g phi1 phi2 ->
+     AnnIso G psi (g_Sym g) phi2 phi1
+ | An_IsoConv : forall (G:context) (psi:grade) (a1 a2 A a1' a2' B:tm) (g:co),
+     AnnDefEq G psi g A B ->
+     AnnPropWff  (meet_ctx_l   q_C    G )   q_C  (Eq a1 a2 A) ->
+     AnnPropWff  (meet_ctx_l   q_C    G )   q_C  (Eq a1' a2' B) ->
       (  (erase_tm  a1 )   =   (erase_tm  a1' )  )  ->
       (  (erase_tm  a2 )   =   (erase_tm  a2' )  )  ->
-     AnnIso G D (g_IsoConv  ( (Eq a1 a2 A) )   ( (Eq a1' a2' B) )  g)  ( (Eq a1 a2 A) )   ( (Eq a1' a2' B) ) 
-with AnnDefEq : context -> available_props -> co -> tm -> tm -> Prop :=    (* defn AnnDefEq *)
- | An_Assn : forall (G:context) (D:available_props) (c:covar) (a b A:tm),
+     AnnIso G psi (g_IsoConv  ( (Eq a1 a2 A) )   ( (Eq a1' a2' B) )  g)  ( (Eq a1 a2 A) )   ( (Eq a1' a2' B) ) 
+with AnnDefCEq : context -> grade -> grade -> co -> tm -> tm -> Prop :=    (* defn AnnDefCEq *)
+with AnnDefEq : context -> grade -> co -> tm -> tm -> Prop :=    (* defn AnnDefEq *)
+ | An_Assn : forall (G:context) (psi:grade) (c:covar) (a b:tm) (psi0:grade) (A:tm),
      AnnCtx G ->
-      binds  c  (Co  (Eq a b A) )  G  ->
-      AtomSetImpl.In  c   D  ->
-     AnnDefEq G D (g_Var_f c) a b
- | An_Refl : forall (G:context) (D:available_props) (a A:tm),
-     AnnTyping G a A ->
-     AnnDefEq G D (g_Refl a) a a
- | An_EraseEq : forall (G:context) (D:available_props) (a b:tm) (g:co) (A B:tm),
-     AnnTyping G a A ->
-     AnnTyping G b B ->
+      ( psi0  <=  psi )  ->
+      binds  c  ( psi0 , (Co  (Eq a b A) ))  G  ->
+     AnnDefEq G psi (g_Var_f c) a b
+ | An_Refl : forall (G:context) (psi:grade) (a A:tm),
+     AnnTyping G psi a A ->
+     AnnDefEq G psi (g_Refl a) a a
+ | An_EraseEq : forall (G:context) (psi:grade) (a b:tm) (g:co) (A B:tm),
+     AnnTyping G psi a A ->
+     AnnTyping G psi b B ->
       (  (erase_tm  a )   =   (erase_tm  b )  )  ->
-     AnnDefEq G  (dom  G )  g A B ->
-     AnnDefEq G D (g_Refl2 a b g) a b
- | An_Sym : forall (G:context) (D:available_props) (g:co) (a b B A:tm) (g1:co),
-     AnnTyping G b B ->
-     AnnTyping G a A ->
-      ( AnnDefEq G  (dom  G )  g1 B A )  ->
-     AnnDefEq G D g b a ->
-     AnnDefEq G D (g_Sym g) a b
- | An_Trans : forall (G:context) (D:available_props) (g1 g2:co) (a b a1 A A1:tm) (g3:co),
-     AnnDefEq G D g1 a a1 ->
-     AnnDefEq G D g2 a1 b ->
-      ( AnnTyping G a A )  ->
-      ( AnnTyping G a1 A1 )  ->
-      ( AnnDefEq G  (dom  G )  g3 A A1 )  ->
-     AnnDefEq G D  ( (g_Trans g1 g2) )  a b
- | An_Beta : forall (G:context) (D:available_props) (a1 a2 B0 B1:tm),
-     AnnTyping G a1 B0 ->
-     AnnTyping G a2 B1 ->
+     AnnDefEq  (meet_ctx_l   q_C    G )   q_C  g A B ->
+     AnnDefEq G psi (g_Refl2 a b g) a b
+ | An_Sym : forall (G:context) (psi:grade) (g:co) (a b B A:tm) (g1:co),
+     AnnTyping G psi b B ->
+     AnnTyping G psi a A ->
+      ( AnnDefEq  (meet_ctx_l   q_C    G )   q_C  g1 B A )  ->
+     AnnDefEq G psi g b a ->
+     AnnDefEq G psi (g_Sym g) a b
+ | An_Trans : forall (G:context) (psi:grade) (g1 g2:co) (a b a1 A A1:tm) (g3:co),
+     AnnDefEq G psi g1 a a1 ->
+     AnnDefEq G psi g2 a1 b ->
+      ( AnnTyping G psi a A )  ->
+      ( AnnTyping G psi a1 A1 )  ->
+      ( AnnDefEq  (meet_ctx_l   q_C    G )   q_C  g3 A A1 )  ->
+     AnnDefEq G psi  ( (g_Trans g1 g2) )  a b
+ | An_Beta : forall (G:context) (psi:grade) (a1 a2 B0 B1:tm),
+     AnnTyping G psi a1 B0 ->
+     AnnTyping G psi a2 B1 ->
       (  (erase_tm  B0 )   =   (erase_tm  B1 )  )  ->
      Beta  (erase_tm  a1 )   (erase_tm  a2 )  ->
-     AnnDefEq G D (g_Beta a1 a2) a1 a2
- | An_PiCong : forall (L:vars) (G:context) (D:available_props) (rho:relflag) (g1 g2:co) (A1 B1 A2 B3 B2:tm),
-     AnnDefEq G D g1 A1 A2 ->
-      ( forall x , x \notin  L  -> AnnDefEq  (( x ~ Tm  A1 ) ++  G )  D  ( open_co_wrt_tm g2 (a_Var_f x) )   ( open_tm_wrt_tm B1 (a_Var_f x) )    (open_tm_wrt_tm  B2   (a_Var_f x) )   )  ->
+     AnnDefEq G psi (g_Beta a1 a2) a1 a2
+ | An_PiCong : forall (L:vars) (G:context) (psi psi0:grade) (g1 g2:co) (A1 B1 A2 B3 B2:tm),
+     AnnDefEq G psi g1 A1 A2 ->
+      ( forall x , x \notin  L  -> AnnDefEq  (( x ~ ( psi , Tm  A1 )) ++  G )  psi  ( open_co_wrt_tm g2 (a_Var_f x) )   ( open_tm_wrt_tm B1 (a_Var_f x) )    (open_tm_wrt_tm  B2   (a_Var_f x) )   )  ->
       ( forall x , x \notin  L  ->  (  ( open_tm_wrt_tm B3 (a_Var_f x) )   =   (open_tm_wrt_tm  B2   (a_Conv (a_Var_f x) (g_Sym g1)) )  )  )  ->
-     AnnTyping G (a_Pi rho A1 B1) a_Star ->
-     AnnTyping G (a_Pi rho A2 B3) a_Star ->
-     AnnTyping G  ( (a_Pi rho A1 B2) )  a_Star ->
-     AnnDefEq G D (g_PiCong rho g1 g2)  ( (a_Pi rho A1 B1) )   ( (a_Pi rho A2 B3) ) 
- | An_AbsCong : forall (L:vars) (G:context) (D:available_props) (rho:relflag) (g1 g2:co) (A1 b1 A2 b3 b2 B:tm),
-     AnnDefEq G D g1 A1 A2 ->
-      ( forall x , x \notin  L  -> AnnDefEq  (( x ~ Tm  A1 ) ++  G )  D  ( open_co_wrt_tm g2 (a_Var_f x) )   ( open_tm_wrt_tm b1 (a_Var_f x) )    (open_tm_wrt_tm  b2   (a_Var_f x) )   )  ->
+     AnnTyping G psi (a_Pi psi0 A1 B1) a_Star ->
+     AnnTyping G psi (a_Pi psi0 A2 B3) a_Star ->
+     AnnTyping G psi  ( (a_Pi psi0 A1 B2) )  a_Star ->
+     AnnDefEq G psi (g_PiCong psi0 g1 g2)  ( (a_Pi psi0 A1 B1) )   ( (a_Pi psi0 A2 B3) ) 
+ | An_AbsCong : forall (L:vars) (G:context) (psi psi0:grade) (g1 g2:co) (A1 b1 A2 b3 b2 B:tm),
+     AnnDefEq  (meet_ctx_l   q_C    G )   q_C  g1 A1 A2 ->
+      ( forall x , x \notin  L  -> AnnDefEq  (( x ~ ( psi0 , Tm  A1 )) ++  G )  psi  ( open_co_wrt_tm g2 (a_Var_f x) )   ( open_tm_wrt_tm b1 (a_Var_f x) )    (open_tm_wrt_tm  b2   (a_Var_f x) )   )  ->
       ( forall x , x \notin  L  ->  (  ( open_tm_wrt_tm b3 (a_Var_f x) )   =   (open_tm_wrt_tm  b2   (a_Conv (a_Var_f x) (g_Sym g1)) )  )  )  ->
-      ( AnnTyping G A1 a_Star )  ->
-     AnnTyping G A2 a_Star ->
-      ( forall x , x \notin  L  -> RhoCheck rho x  (erase_tm   ( open_tm_wrt_tm b1 (a_Var_f x) )  )  )  ->
-      ( forall x , x \notin  L  -> RhoCheck rho x  (erase_tm   ( open_tm_wrt_tm b3 (a_Var_f x) )  )  )  ->
-      ( AnnTyping G  ( (a_Abs rho A1 b2) )  B )  ->
-     AnnDefEq G D  ( (g_AbsCong rho g1 g2) )   ( (a_Abs rho A1 b1) )   ( (a_Abs rho A2 b3) ) 
- | An_AppCong : forall (G:context) (D:available_props) (g1:co) (rho:relflag) (g2:co) (a1 a2 b1 b2 A B:tm) (g3:co),
-     AnnDefEq G D g1 a1 b1 ->
-     AnnDefEq G D g2 a2 b2 ->
-     AnnTyping G (a_App a1 rho a2) A ->
-     AnnTyping G (a_App b1 rho b2) B ->
-      ( AnnDefEq G  (dom  G )  g3 A B )  ->
-     AnnDefEq G D (g_AppCong g1 rho g2) (a_App a1 rho a2) (a_App b1 rho b2)
- | An_PiFst : forall (G:context) (D:available_props) (g:co) (A1 A2:tm) (rho:relflag) (B1 B2:tm),
-     AnnDefEq G D g (a_Pi rho A1 B1) (a_Pi rho A2 B2) ->
-     AnnDefEq G D (g_PiFst g) A1 A2
- | An_PiSnd : forall (G:context) (D:available_props) (g1 g2:co) (B1 a1 B2 a2:tm) (rho:relflag) (A1 A2:tm),
-     AnnDefEq G D g1 (a_Pi rho A1 B1) (a_Pi rho A2 B2) ->
-     AnnDefEq G D g2 a1 a2 ->
-     AnnTyping G a1 A1 ->
-     AnnTyping G a2 A2 ->
-     AnnDefEq G D (g_PiSnd g1 g2)   (open_tm_wrt_tm  B1   a1 )     (open_tm_wrt_tm  B2   a2 )  
- | An_CPiCong : forall (L:vars) (G:context) (D:available_props) (g1 g3:co) (phi1:constraint) (B1:tm) (phi2:constraint) (B3 B2:tm),
-     AnnIso G D g1 phi1 phi2 ->
-      ( forall c , c \notin  L  -> AnnDefEq  (( c ~ Co  phi1 ) ++  G )  D  ( open_co_wrt_co g3 (g_Var_f c) )   ( open_tm_wrt_co B1 (g_Var_f c) )    (open_tm_wrt_co  B2   (g_Var_f c) )   )  ->
+      ( AnnTyping  (meet_ctx_l   q_C    G )   q_C  A1 a_Star )  ->
+     AnnTyping  (meet_ctx_l   q_C    G )   q_C  A2 a_Star ->
+      ( AnnTyping G psi (a_Abs psi0 A1 b2) B )  ->
+     AnnDefEq G psi  ( (g_AbsCong psi0 g1 g2) )   ( (a_Abs psi0 A1 b1) )   ( (a_Abs psi0 A2 b3) ) 
+ | An_AppCong : forall (G:context) (psi:grade) (g1:co) (psi0:grade) (g2:co) (a1 a2 b1 b2 A B:tm) (g3:co),
+     AnnDefEq G psi g1 a1 b1 ->
+     AnnDefCEq G psi psi0 g2 a2 b2 ->
+     AnnTyping G psi (a_App a1 psi0 a2) A ->
+     AnnTyping G psi (a_App b1 psi0 b2) B ->
+      ( AnnDefEq  (meet_ctx_l   q_C    G )   q_C  g3 A B )  ->
+     AnnDefEq G psi (g_AppCong g1 psi0 g2) (a_App a1 psi0 a2) (a_App b1 psi0 b2)
+ | An_PiFst : forall (G:context) (psi:grade) (g:co) (A1 A2:tm) (psi0:grade) (B1 B2:tm),
+     AnnDefEq G psi g (a_Pi psi0 A1 B1) (a_Pi psi0 A2 B2) ->
+     AnnDefEq G psi (g_PiFst g) A1 A2
+ | An_PiSnd : forall (G:context) (psi:grade) (g1 g2:co) (B1 a1 B2 a2:tm) (psi0:grade) (A1 A2:tm),
+     AnnDefEq G psi g1 (a_Pi psi0 A1 B1) (a_Pi psi0 A2 B2) ->
+     AnnDefEq G psi g2 a1 a2 ->
+     AnnTyping G psi a1 A1 ->
+     AnnTyping G psi a2 A2 ->
+     AnnDefEq G psi (g_PiSnd g1 g2)   (open_tm_wrt_tm  B1   a1 )     (open_tm_wrt_tm  B2   a2 )  
+ | An_CPiCong : forall (L:vars) (G:context) (psi:grade) (g1 g3:co) (psi0:grade) (phi1:constraint) (B1:tm) (phi2:constraint) (B3 B2:tm),
+     AnnIso G psi g1 phi1 phi2 ->
+      ( forall c , c \notin  L  -> AnnDefEq  (( c ~ ( psi , Co  phi1 )) ++  G )  psi  ( open_co_wrt_co g3 (g_Var_f c) )   ( open_tm_wrt_co B1 (g_Var_f c) )    (open_tm_wrt_co  B2   (g_Var_f c) )   )  ->
       ( forall c , c \notin  L  ->  (  ( open_tm_wrt_co B3 (g_Var_f c) )   =   (open_tm_wrt_co  B2   (g_Cast (g_Var_f c) (g_Sym g1)) )  )  )  ->
-     AnnTyping G (a_CPi phi1 B1) a_Star ->
-      ( AnnTyping G (a_CPi phi2 B3) a_Star )  ->
-     AnnTyping G (a_CPi phi1 B2) a_Star ->
-     AnnDefEq G D  ( (g_CPiCong g1 g3) )   ( (a_CPi phi1 B1) )   ( (a_CPi phi2 B3) ) 
- | An_CAbsCong : forall (L:vars) (G:context) (D:available_props) (g1 g3 g4:co) (phi1:constraint) (a1:tm) (phi2:constraint) (a3 a2 B1 B2 B:tm),
-     AnnIso G D g1 phi1 phi2 ->
-      ( forall c , c \notin  L  -> AnnDefEq  (( c ~ Co  phi1 ) ++  G )  D  ( open_co_wrt_co g3 (g_Var_f c) )   ( open_tm_wrt_co a1 (g_Var_f c) )    (open_tm_wrt_co  a2   (g_Var_f c) )   )  ->
+     AnnTyping G psi (a_CPi psi0 phi1 B1) a_Star ->
+      ( AnnTyping G psi (a_CPi psi0 phi2 B3) a_Star )  ->
+     AnnTyping G psi (a_CPi psi0 phi1 B2) a_Star ->
+     AnnDefEq G psi  ( (g_CPiCong g1 g3) )   ( (a_CPi psi0 phi1 B1) )   ( (a_CPi psi0 phi2 B3) ) 
+ | An_CAbsCong : forall (L:vars) (G:context) (psi psi0:grade) (g1 g3 g4:co) (phi1:constraint) (a1:tm) (phi2:constraint) (a3 a2 B1 B2 B:tm),
+     AnnIso G psi g1 phi1 phi2 ->
+      ( forall c , c \notin  L  -> AnnDefEq  (( c ~ (  (q_join  psi0   psi )  , Co  phi1 )) ++  G )  psi  ( open_co_wrt_co g3 (g_Var_f c) )   ( open_tm_wrt_co a1 (g_Var_f c) )    (open_tm_wrt_co  a2   (g_Var_f c) )   )  ->
       ( forall c , c \notin  L  ->  (  ( open_tm_wrt_co a3 (g_Var_f c) )   =   (open_tm_wrt_co  a2   (g_Cast (g_Var_f c) (g_Sym g1)) )  )  )  ->
-     AnnTyping G  ( (a_CAbs phi1 a1) )  (a_CPi phi1 B1) ->
-     AnnTyping G  ( (a_CAbs phi2 a3) )  (a_CPi phi2 B2) ->
-     AnnTyping G  ( (a_CAbs phi1 a2) )  B ->
-     AnnDefEq G  (dom  G )  g4 (a_CPi phi1 B1) (a_CPi phi2 B2) ->
-     AnnDefEq G D  ( (g_CAbsCong g1 g3 g4) )   ( (a_CAbs phi1 a1) )   ( (a_CAbs phi2 a3) ) 
- | An_CAppCong : forall (G:context) (D:available_props) (g1 g2 g3:co) (a1 b1 a2 b2 a3 b3 A B:tm) (g4:co),
-     AnnDefEq G D g1 a1 b1 ->
-     AnnDefEq G  (dom  G )  g2 a2 b2 ->
-     AnnDefEq G  (dom  G )  g3 a3 b3 ->
-     AnnTyping G (a_CApp a1 g2) A ->
-     AnnTyping G (a_CApp b1 g3) B ->
-      ( AnnDefEq G  (dom  G )  g4 A B )  ->
-     AnnDefEq G D (g_CAppCong g1 g2 g3) (a_CApp a1 g2) (a_CApp b1 g3)
- | An_CPiSnd : forall (G:context) (D:available_props) (g1 g2 g3:co) (B1 B2 a a' A b b' B:tm),
-     AnnDefEq G D g1  ( (a_CPi (Eq a a' A) B1) )   ( (a_CPi (Eq b b' B) B2) )  ->
-     AnnDefEq G  (dom  G )  g2 a a' ->
-     AnnDefEq G  (dom  G )  g3 b b' ->
-     AnnDefEq G D (g_CPiSnd g1 g2 g3)  (open_tm_wrt_co  B1   g2 )   (open_tm_wrt_co  B2   g3 ) 
- | An_Cast : forall (G:context) (D:available_props) (g1 g2:co) (b b' a a' A B:tm),
-     AnnDefEq G D g1 a a' ->
-     AnnIso G D g2 (Eq a a' A) (Eq b b' B) ->
-     AnnDefEq G D (g_Cast g1 g2) b b'
- | An_IsoSnd : forall (G:context) (D:available_props) (g:co) (A B a a' b b':tm),
-     AnnIso G D g  ( (Eq a a' A) )   ( (Eq b b' B) )  ->
-     AnnDefEq G D (g_IsoSnd g) A B
- | An_Eta : forall (L:vars) (G:context) (D:available_props) (b:tm) (rho:relflag) (A a B:tm),
-     AnnTyping G b (a_Pi rho A B) ->
-      ( forall x , x \notin  L  ->  (  ( open_tm_wrt_tm a (a_Var_f x) )   =  (a_App b rho (a_Var_f x)) )  )  ->
-     AnnDefEq G D (g_Eta b)  ( (a_Abs rho A a) )  b
- | An_EtaC : forall (L:vars) (G:context) (D:available_props) (b:tm) (phi:constraint) (a B:tm),
-     AnnTyping G b (a_CPi phi B) ->
+     AnnTyping G psi  ( (a_CAbs psi0 phi1 a1) )  (a_CPi psi0 phi1 B1) ->
+     AnnTyping G psi  ( (a_CAbs psi0 phi2 a3) )  (a_CPi psi0 phi2 B2) ->
+     AnnTyping G psi  ( (a_CAbs psi0 phi1 a2) )  B ->
+     AnnDefEq  (meet_ctx_l   q_C    G )  psi g4 (a_CPi psi0 phi1 B1) (a_CPi psi0 phi2 B2) ->
+     AnnDefEq G psi  ( (g_CAbsCong psi0 g1 g3 g4) )   ( (a_CAbs psi0 phi1 a1) )   ( (a_CAbs psi0 phi2 a3) ) 
+ | An_CAppCong : forall (G:context) (psi:grade) (g1 g2 g3:co) (a1 b1 a2 b2 a3 b3 A B:tm) (g4:co),
+     AnnDefEq G psi g1 a1 b1 ->
+     AnnDefEq  (meet_ctx_l   q_C    G )   q_C  g2 a2 b2 ->
+     AnnDefEq  (meet_ctx_l   q_C    G )   q_C  g3 a3 b3 ->
+     AnnTyping G psi (a_CApp a1 g2) A ->
+     AnnTyping G psi (a_CApp b1 g3) B ->
+      ( AnnDefEq  (meet_ctx_l   q_C    G )   q_C  g4 A B )  ->
+     AnnDefEq G psi (g_CAppCong g1 g2 g3) (a_CApp a1 g2) (a_CApp b1 g3)
+ | An_CPiSnd : forall (G:context) (psi:grade) (g1 g2 g3:co) (B1 B2:tm) (psi0:grade) (a a' A b b' B:tm),
+     AnnDefEq G psi g1  ( (a_CPi psi0 (Eq a a' A) B1) )   ( (a_CPi psi0 (Eq b b' B) B2) )  ->
+     AnnDefEq  (meet_ctx_l   q_C    G )   q_C  g2 a a' ->
+     AnnDefEq  (meet_ctx_l   q_C    G )   q_C  g3 b b' ->
+     AnnDefEq G psi (g_CPiSnd g1 g2 g3)  (open_tm_wrt_co  B1   g2 )   (open_tm_wrt_co  B2   g3 ) 
+ | An_Cast : forall (G:context) (psi:grade) (g1 g2:co) (b b' a a' A B:tm),
+     AnnDefEq G psi g1 a a' ->
+     AnnIso G psi g2 (Eq a a' A) (Eq b b' B) ->
+     AnnDefEq G psi (g_Cast g1 g2) b b'
+ | An_IsoSnd : forall (G:context) (psi:grade) (g:co) (A B a a' b b':tm),
+     AnnIso G psi g  ( (Eq a a' A) )   ( (Eq b b' B) )  ->
+     AnnDefEq G psi (g_IsoSnd g) A B
+ | An_Eta : forall (L:vars) (G:context) (psi:grade) (b:tm) (psi0:grade) (A a B:tm),
+     AnnTyping G psi b (a_Pi psi0 A B) ->
+      ( forall x , x \notin  L  ->  (  ( open_tm_wrt_tm a (a_Var_f x) )   =  (a_App b psi0 (a_Var_f x)) )  )  ->
+     AnnDefEq G psi (g_Eta b)  ( (a_Abs psi0 A a) )  b
+ | An_EtaC : forall (L:vars) (G:context) (psi:grade) (b:tm) (psi0:grade) (phi:constraint) (a B:tm),
+     AnnTyping G psi b (a_CPi psi0 phi B) ->
       ( forall c , c \notin  L  ->  (  ( open_tm_wrt_co a (g_Var_f c) )   =  (a_CApp b (g_Var_f c)) )  )  ->
-     AnnDefEq G D (g_Eta b)  ( (a_CAbs phi a) )  b
+     AnnDefEq G psi (g_Eta b)  ( (a_CAbs psi0 phi a) )  b
 with AnnCtx : context -> Prop :=    (* defn AnnCtx *)
  | An_Empty : 
      AnnCtx  nil 
- | An_ConsTm : forall (G:context) (x:tmvar) (A:tm),
+ | An_ConsTm : forall (G:context) (x:tmvar) (psi0:grade) (A:tm),
      AnnCtx G ->
-     AnnTyping G A a_Star ->
+     AnnTyping  (meet_ctx_l   q_C    G )   q_C  A a_Star ->
       ~ AtomSetImpl.In  x  (dom  G )  ->
-     AnnCtx  (( x ~ Tm  A ) ++  G ) 
- | An_ConsCo : forall (G:context) (c:covar) (phi:constraint),
+     AnnCtx  (( x ~ ( psi0 , Tm  A )) ++  G ) 
+ | An_ConsCo : forall (G:context) (c:covar) (psi0:grade) (phi:constraint),
      AnnCtx G ->
-     AnnPropWff G phi ->
+     AnnPropWff  (meet_ctx_l   q_C    G )   q_C  phi ->
       ~ AtomSetImpl.In  c  (dom  G )  ->
-     AnnCtx  (( c ~ Co  phi ) ++  G ) 
+     AnnCtx  (( c ~ ( psi0 , Co  phi )) ++  G ) 
 with AnnSig : sig -> Prop :=    (* defn AnnSig *)
  | An_Sig_Empty : 
      AnnSig  nil 
  | An_Sig_ConsAx : forall (S:sig) (F:tyfam) (a A:tm),
      AnnSig S ->
-     AnnTyping  nil  A a_Star ->
-     AnnTyping  nil  a A ->
+     AnnTyping  nil   q_C  A a_Star ->
+     AnnTyping  nil   q_C  a A ->
       ~ AtomSetImpl.In  F  (dom  S )  ->
      AnnSig  (( F ~ Ax a A )++ S ) .
 
 (* defns Jred *)
 Inductive head_reduction : context -> tm -> tm -> Prop :=    (* defn head_reduction *)
- | An_AppLeft : forall (G:context) (a:tm) (rho:relflag) (b a':tm),
+ | An_AppLeft : forall (G:context) (a:tm) (psi0:grade) (b a':tm),
      lc_tm b ->
      head_reduction G a a' ->
-     head_reduction G (a_App a rho b) (a_App a' rho b)
- | An_AppAbs : forall (G:context) (rho:relflag) (A w a:tm),
+     head_reduction G (a_App a psi0 b) (a_App a' psi0 b)
+ | An_AppAbs : forall (G:context) (psi0:grade) (A w a:tm),
      lc_tm a ->
-     Value  ( (a_Abs rho A w) )  ->
-     head_reduction G (a_App  ( (a_Abs rho A w) )  rho a)  (open_tm_wrt_tm  w   a ) 
+     Value  ( (a_Abs psi0 A w) )  ->
+     head_reduction G (a_App  ( (a_Abs psi0 A w) )  psi0 a)  (open_tm_wrt_tm  w   a ) 
  | An_CAppLeft : forall (G:context) (a:tm) (g:co) (a':tm),
      lc_co g ->
      head_reduction G a a' ->
      head_reduction G (a_CApp a g) (a_CApp a' g)
- | An_CAppCAbs : forall (G:context) (phi:constraint) (b:tm) (g:co),
+ | An_CAppCAbs : forall (G:context) (psi0:grade) (phi:constraint) (b:tm) (g:co),
      lc_constraint phi ->
-     lc_tm (a_CAbs phi b) ->
+     lc_tm (a_CAbs psi0 phi b) ->
      lc_co g ->
-     head_reduction G (a_CApp  ( (a_CAbs phi b) )  g)  (open_tm_wrt_co  b   g ) 
- | An_AbsTerm : forall (L:vars) (G:context) (A b b':tm),
-     AnnTyping G A a_Star ->
-      ( forall x , x \notin  L  -> head_reduction  (( x ~ Tm  A ) ++  G )   ( open_tm_wrt_tm b (a_Var_f x) )   ( open_tm_wrt_tm b' (a_Var_f x) )  )  ->
-     head_reduction G  ( (a_Abs Irrel A b) )   ( (a_Abs Irrel A b') ) 
+     head_reduction G (a_CApp  ( (a_CAbs psi0 phi b) )  g)  (open_tm_wrt_co  b   g ) 
  | An_Axiom : forall (G:context) (F:tyfam) (a A:tm),
       binds  F  (Ax  a A )   an_toplevel   ->
      head_reduction G (a_Fam F) a
@@ -1510,21 +1646,21 @@ Inductive head_reduction : context -> tm -> tm -> Prop :=    (* defn head_reduct
      lc_co g2 ->
      Value v ->
      head_reduction G (a_Conv  ( (a_Conv v g1) )  g2) (a_Conv v  ( (g_Trans g1 g2) ) )
- | An_Push : forall (G:context) (v:tm) (g:co) (rho:relflag) (b b':tm) (g':co) (A1 B1 A2 B2:tm),
+ | An_Push : forall (G:context) (v:tm) (g:co) (psi0:grade) (b b':tm) (g':co) (psi:grade) (A1 B1 A2 B2:tm),
      Value v ->
-     AnnDefEq G  (dom  G )  g (a_Pi rho A1 B1) (a_Pi rho A2 B2) ->
+     AnnDefEq  (meet_ctx_l   q_C    G )  psi g (a_Pi psi0 A1 B1) (a_Pi psi0 A2 B2) ->
       ( b'  =  (a_Conv b (g_Sym  ( (g_PiFst g) ) )) )  ->
       ( g'  =  (g_PiSnd g (g_Refl2 b' b  ( (g_PiFst g) ) )) )  ->
-     head_reduction G (a_App  ( (a_Conv v g) )  rho b) (a_Conv  ( (a_App v rho b') )  g')
- | An_CPush : forall (G:context) (v:tm) (g g1 g1' g':co) (phi1:constraint) (A1:tm) (phi2:constraint) (A2:tm),
+     head_reduction G (a_App  ( (a_Conv v g) )  psi0 b) (a_Conv  ( (a_App v psi0 b') )  g')
+ | An_CPush : forall (G:context) (v:tm) (g g1 g1' g':co) (psi psi0:grade) (phi1:constraint) (A1:tm) (phi2:constraint) (A2:tm),
      Value v ->
-     AnnDefEq G  (dom  G )  g (a_CPi phi1 A1) (a_CPi phi2 A2) ->
+     AnnDefEq  (meet_ctx_l   q_C    G )  psi g (a_CPi psi0 phi1 A1) (a_CPi psi0 phi2 A2) ->
       ( g1'  =  (g_Cast g1 (g_Sym  ( (g_CPiFst g) ) )) )  ->
       ( g'  =  (g_CPiSnd g g1' g1) )  ->
      head_reduction G (a_CApp  ( (a_Conv v g) )  g1) (a_Conv  ( (a_CApp v g1') )  g').
 
 
 (** infrastructure *)
-Hint Constructors CoercedValue Value value_type consistent RhoCheck erased_constraint erased_tm ParProp Par multipar multipar_prop Beta reduction_in_one reduction PropWff Typing Iso DefEq Ctx Sig AnnPropWff AnnTyping AnnIso AnnDefEq AnnCtx AnnSig head_reduction lc_co lc_brs lc_tm lc_constraint lc_sort lc_sig_sort : core.
+Hint Constructors CoercedValue Value value_type consistent erased_constraint erased_tm P_sub ctx_sub CoGrade CGrade Grade CoGEq CEq GEq CParProp CPar ParProp Par multipar multipar_prop Beta reduction_in_one reduction PropWff Typing Iso CDefEq DefEq Ctx Sig AnnPropWff AnnTyping AnnIso AnnDefCEq AnnDefEq AnnCtx AnnSig head_reduction lc_co lc_brs lc_tm lc_constraint lc_sig_sort lc_sort : core.
 
 
